Encodings.v
@@ -1,0 +1,156 @@
+Require Import List.
+Require Import ZArith.
+Require Import Lia.
+Require Import FSets.FMapPositive.
+
+From BusyCoq Require Import BB52Statement.
+From BusyCoq Require Import CustomTactics.
+From BusyCoq Require Import Prelims.
+
+
+Fixpoint positive_len(x:positive):nat :=
+match x with
+| xH => O
+| xI x0 => S (positive_len x0)
+| xO x0 => S (positive_len x0)
+end.
+
+Fixpoint enc_v1(x:positive):positive :=
+match x with
+| xH => xH
+| xI x0 => xI (xI (enc_v1 x0))
+| xO x0 => xI (xO (enc_v1 x0))
+end.
+
+Lemma enc_v1_eq a1 b1 a2 b2:
+  append (enc_v1 a1) (xO b1) = append (enc_v1 a2) (xO b2) ->
+  (a1 = a2 /\ b1 = b2).
+Proof.
+  gd a2.
+  induction a1; destruct a2; cbn; intros; cg; invst H.
+  1,2: destruct (IHa1 a2 H1).
+  all: split; cg.
+Qed.
+
+Definition enc_pair(x:positive*positive):positive :=
+  let (x1,x2):=x in
+  append (enc_v1 (Pos.of_succ_nat (positive_len x1))) (xO (append x1 x2)).
+
+Lemma enc_pair_inj: is_inj enc_pair.
+Proof.
+  intros x1 x2 H.
+  destruct x1 as [a1 b1].
+  destruct x2 as [a2 b2].
+  unfold enc_pair in H.
+  destruct (enc_v1_eq _ _ _ _ H) as [Ha Hb]. clear H.
+  assert (positive_len a1 = positive_len a2) by lia. clear Ha.
+  gd a2.
+  induction a1; destruct a2; cbn; intros; cg;
+  invst Hb;
+  invst H;
+  assert ((a1,b1)=(a2,b2)) by auto 2;
+  cg.
+Qed.
+
+
+Fixpoint enc_list(x:list positive):positive :=
+match x with
+| nil => xH
+| h::t => enc_pair (h,enc_list t)
+end.
+
+Lemma enc_list_inj: is_inj enc_list.
+Proof.
+  intros x1 x2 H.
+  gd x2.
+  induction x1 as [|h1 t1]; destruct x2 as [|h2 t2]; intros; cg.
+  - cbn in H. destruct ((Pos.of_succ_nat (positive_len h2))); cbn in H; cg.
+  - cbn in H. destruct ((Pos.of_succ_nat (positive_len h1))); cbn in H; cg.
+  - epose proof (enc_pair_inj _ _ H).
+    invst H0.
+    f_equal.
+    apply IHt1; assumption.
+Qed.
+
+Definition St_enc(x:St):positive :=
+match x with
+| St0 => xH
+| St1 => xO xH
+| St2 => xI xH
+| St3 => xO (xO xH)
+| St4 => xI (xO xH)
+end.
+
+Lemma St_enc_inj: is_inj St_enc.
+  intros x1 x2.
+  destruct x1,x2; cbn; cg.
+Qed.
+
+Definition Σ_eqb(i1 i2:Σ) :=
+match i1,i2 with
+| Σ0,Σ0 | Σ1,Σ1 => true
+| _,_ => false
+end.
+
+Lemma Σ_eqb_spec i1 i2:
+  if Σ_eqb i1 i2 then i1=i2 else i1<>i2.
+Proof.
+  destruct i1,i2; cbn; congruence.
+Qed.
+
+
+
+Definition Σ_enc(x:Σ):positive :=
+match x with
+| Σ0 => xH
+| Σ1 => xO xH
+end.
+
+Lemma Σ_enc_inj: is_inj Σ_enc.
+  intros x1 x2.
+  destruct x1,x2; cbn; cg.
+Qed.
+
+
+Fixpoint listΣ_enc(x:list Σ):positive :=
+match x with
+| nil => xH
+| Σ0::t => xO (listΣ_enc t)
+| Σ1::t => xI (listΣ_enc t)
+end.
+
+Lemma listΣ_inj: is_inj listΣ_enc.
+Proof.
+  intros x1 x2 H.
+  gd x2.
+  induction x1 as [|h1 t1]; destruct x2 as [|h2 t2]; cbn; intros; cg.
+  - destruct h2; invst H.
+  - destruct h1; invst H.
+  - destruct h1,h2; invst H.
+    1,2: f_equal; apply IHt1,H1.
+Qed.
+
+
+
+Lemma map_inj{T1 T2}(f:T1->T2): is_inj f -> is_inj (map f).
+Proof.
+  intros H x1 x2 H0.
+  gd x2.
+  induction x1 as [|h1 t1]; destruct x2 as [|h2 t2]; cbn; intros; cg.
+  invst H0.
+  rewrite (IHt1 _ H3).
+  f_equal.
+  apply H,H2.
+Qed.
+
+Definition listT_enc{T}(f:T->positive)(x:list T):positive :=
+  enc_list (map f x).
+
+Lemma listT_enc_inj{T}(f:T->positive): is_inj f -> is_inj (listT_enc f).
+Proof.
+  intros H x1 x2 H0.
+  unfold listT_enc.
+  apply (map_inj _ H).
+  unfold listT_enc in H0.
+  apply enc_list_inj,H0.
+Qed.
