ListTape.v
@@ -1,0 +1,2357 @@
+Require Import ZArith.
+Require Import List.
+Require Import Lia.
+
+From BusyCoq Require Import Prelims.
+From BusyCoq Require Import Encodings.
+From BusyCoq Require Import TM_CoqBB5.
+From BusyCoq Require Import BB52Statement.
+From BusyCoq Require Import CustomTactics.
+From BusyCoq Require Import CustomListRoutines.
+From BusyCoq Require Import Decider_NGramCPS.
+
+Section ListTape_assumeSigma.
+
+Record ListES := {
+  l: list Σ;
+  r: list Σ;
+  m: Σ;
+  s: St;
+}.
+
+Definition ListES_toES(x:ListES):ExecState Σ :=
+let (l0,r0,m0,s0):=x in
+(s0,
+fun x =>
+match x with
+| Zpos x0 => nth (Pos.to_nat x0) (m0::r0) Σ0
+| Zneg x0 => nth (Pos.to_nat x0) (m0::l0) Σ0
+| Z0 => m0
+end).
+
+Definition ListES_step(tm:TM Σ)(x:ListES):option ListES :=
+let (l0,r0,m0,s0):=x in
+match tm s0 m0 with
+| None => None
+| Some tr =>
+  let (s1,d,o) := tr in
+    Some
+    match d with
+    | Dpos =>
+      match r0 with
+      | m1::r1 => {| l:=o::l0; r:=r1; m:=m1; s:=s1 |}
+      | nil => {| l:=o::l0; r:=nil; m:=Σ0; s:=s1 |}
+      end
+    | Dneg =>
+      match l0 with
+      | m1::l1 => {| l:=l1; r:=o::r0; m:=m1; s:=s1 |}
+      | nil => {| l:=nil; r:=o::r0; m:=Σ0; s:=s1 |}
+      end
+    end
+end.
+
+Lemma ListES_step_spec tm x:
+  step Σ tm (ListES_toES x) =
+  match ListES_step tm x with
+  | None => None
+  | Some x1 => Some (ListES_toES x1)
+  end.
+Proof.
+  destruct x as [l0 r0 m0 s0].
+  cbn.
+  destruct (tm s0 m0) as [[s' d o]|].
+  2: reflexivity.
+  unfold mov,upd.
+  destruct d; cbn.
+  + destruct l0; cbn.
+    * f_equal. f_equal. fext.
+      assert (H:(x<0\/x=0\/x=1\/x>1)%Z) by lia.
+      destruct H as [H|[H|[H|H]]].
+      -- destruct x; try lia.
+         destruct ((Z.neg p + -1)%Z) eqn:E; cbn; try lia.
+         destruct (Pos.to_nat p0) eqn:E0. 1: lia.
+         destruct n,(Pos.to_nat p); auto 1.
+         ++ destruct n; reflexivity.
+         ++ destruct n0; reflexivity.
+      -- subst. reflexivity.
+      -- subst. reflexivity.
+      -- destruct x; try lia.
+         destruct ((Z.pos p + -1)%Z) eqn:E; cbn; try lia.
+         destruct (Pos.to_nat p0) eqn:E0. 1: lia.
+         assert (Pos.to_nat p = S (S n)) by lia. rewrite H0. reflexivity.
+    * f_equal. f_equal. fext.
+      assert (H:(x<0\/x=0\/x=1\/x>1)%Z) by lia.
+      destruct H as [H|[H|[H|H]]].
+      -- destruct x; try lia.
+         destruct ((Z.neg p + -1)%Z) eqn:E; cbn; try lia.
+         destruct (Pos.to_nat p0) eqn:E0. 1: lia.
+         assert (n=Pos.to_nat p) by lia. rewrite H0. reflexivity.
+      -- subst. reflexivity.
+      -- subst. reflexivity.
+      -- destruct x; try lia.
+         destruct ((Z.pos p + -1)%Z) eqn:E; cbn; try lia.
+         destruct (Pos.to_nat p0) eqn:E0. 1: lia.
+         assert (Pos.to_nat p = S (S n)) by lia. rewrite H0. reflexivity.
+  + destruct r0; cbn.
+    * f_equal. f_equal. fext.
+      assert (H:(x>0\/x=0\/x=-1\/x<(-1))%Z) by lia.
+      destruct H as [H|[H|[H|H]]].
+      -- destruct x; try lia.
+         destruct ((Z.neg p + -1)%Z) eqn:E; cbn; try lia.
+         destruct (Pos.to_nat p0) eqn:E0. 1: lia.
+         destruct (Pos.to_nat (p + 1)) eqn:E1; try lia.
+         destruct n0,(Pos.to_nat p); auto 1.
+         ++ destruct n0; reflexivity.
+         ++ destruct n1; reflexivity.
+      -- subst. reflexivity.
+      -- subst. reflexivity.
+      -- destruct x; try lia.
+         destruct ((Z.neg p + 1)%Z) eqn:E; cbn; try lia.
+         destruct (Pos.to_nat p0) eqn:E0. 1: lia.
+         assert (Pos.to_nat p = S (S n)) by lia. rewrite H0. reflexivity.
+    * f_equal. f_equal. fext.
+      assert (H:(x>0\/x=0\/x=-1\/x<(-1))%Z) by lia.
+      destruct H as [H|[H|[H|H]]].
+      -- destruct x; try lia.
+         destruct ((Z.pos p + 1)%Z) eqn:E; cbn; try lia.
+         destruct (Pos.to_nat p) eqn:E0. 1: lia.
+         assert (Pos.to_nat p0 = S (S n)) by lia. rewrite H0. reflexivity.
+      -- subst. reflexivity.
+      -- subst. reflexivity.
+      -- destruct x; try lia.
+         destruct ((Z.neg p + 1)%Z) eqn:E; cbn; try lia.
+         destruct (Pos.to_nat p) eqn:E0. 1: lia.
+         assert (n=Pos.to_nat p0) by lia. rewrite <-H0.
+         destruct n. 1: lia. reflexivity.
+Qed.
+
+
+Definition app_halftape(h:list Σ)(t:nat->Σ):nat->Σ :=
+  fun n =>
+  match nth_error h n with
+  | None => t (n-(length h))
+  | Some c => c
+  end.
+
+Definition make_tape(l0:nat->Σ)(m0:Σ)(r0:nat->Σ):Z->Σ :=
+  fun x =>
+  match x with
+  | Z0 => m0
+  | Zpos x0 => r0 (Nat.pred (Pos.to_nat x0))
+  | Zneg x0 => l0 (Nat.pred (Pos.to_nat x0))
+  end.
+
+Definition make_tape'(l1:nat->Σ)(l0:list Σ)(m0:Σ)(r0:list Σ)(r1:nat->Σ):Z->Σ :=
+  make_tape (app_halftape l0 l1) m0 (app_halftape r0 r1).
+
+Definition makeES(st:ListES)(l1 r1:nat->Σ):ExecState Σ :=
+  let (l0,r0,m0,s0):=st in
+  (s0, make_tape' l1 l0 m0 r0 r1).
+
+Definition addmul(x:Z)(d:Dir)(n:nat):Z := x+(Dir_to_Z d)*(Z.of_nat n).
+
+Definition half_tape(f:Z->Σ)(x:Z)(d:Dir):nat->Σ :=
+  fun n =>
+  f (addmul x d n).
+
+Lemma make_tape'_spec (t:Z->Σ) nl nr:
+  t = 
+  make_tape'
+    (half_tape t (-Z.of_nat(1+nl))%Z Dneg)
+    (tape_seg _ t ((-1)%Z) Dneg nl)
+    (t Z0)
+    (tape_seg _ t (1%Z) Dpos nr)
+    (half_tape t (Z.of_nat (1+nr)) Dpos).
+Proof.
+  fext.
+  cbn.
+  destruct x.
+  - cbn. reflexivity.
+  - cbn.
+    unfold app_halftape.
+    remember (Nat.pred (Pos.to_nat p)) as p0.
+    destruct (tape_seg_spec Σ t 1 Dpos nr) as [H0 H1].
+    assert (H:p0<nr\/nr<=p0) by lia.
+    destruct H as [H|H].
+    + rewrite H0; auto 1. f_equal.
+      unfold Dir_to_Z. subst. lia.
+    + pose proof H as H2.
+      rewrite <-H1 in H.
+      rewrite <-nth_error_None in H.
+      rewrite H.
+      unfold half_tape.
+      f_equal.
+      unfold addmul,Dir_to_Z.
+      lia.
+  - cbn.
+    unfold app_halftape.
+    remember (Nat.pred (Pos.to_nat p)) as p0.
+    destruct (tape_seg_spec Σ t (-1) Dneg nl) as [H0 H1].
+    assert (H:p0<nl\/nl<=p0) by lia.
+    destruct H as [H|H].
+    + rewrite H0; auto 1. f_equal.
+      unfold Dir_to_Z. subst. lia.
+    + pose proof H as H2.
+      rewrite <-H1 in H.
+      rewrite <-nth_error_None in H.
+      rewrite H.
+      unfold half_tape.
+      f_equal.
+      unfold addmul,Dir_to_Z.
+      lia.
+Qed.
+
+Lemma make_tape'_lmr (t:Z->Σ):
+  t = 
+  make_tape'
+    (half_tape t (-1) Dneg)
+    nil
+    (t Z0)
+    nil
+    (half_tape t 1 Dpos).
+Proof.
+  apply (make_tape'_spec t 0 0).
+Qed.
+
+Lemma make_tape'_upd l1' l1 m1 r1 r1' m1':
+  upd Σ (make_tape' l1' l1 m1 r1 r1') m1' = (make_tape' l1' l1 m1' r1 r1').
+Proof.
+  fext.
+  unfold upd.
+  destruct x; cbn; reflexivity.
+Qed.
+
+Lemma app_halftape_S m1 l1 l1' n:
+  app_halftape (m1 :: l1) l1' (S n) = app_halftape l1 l1' n.
+Proof.
+  unfold app_halftape. cbn. reflexivity.
+Qed.
+
+Lemma make_tape'_mov_l l1' l1 m1 r1 r1' σ:
+  mov Σ (make_tape' l1' (σ :: l1) m1 r1 r1') Dneg = make_tape' l1' l1 σ (m1 :: r1) r1'.
+Proof.
+  fext.
+  unfold mov,make_tape',make_tape,Dir_to_Z.
+  assert (H:(x<0\/x=0\/x=1\/x>1)%Z) by lia.
+  destruct H as [H|[H|[H|H]]].
+  - destruct x; try lia.
+    destruct (Z.neg p + -1)%Z eqn:E; try lia.
+    assert (H0:(Nat.pred (Pos.to_nat p0)) = S (Nat.pred (Pos.to_nat p))) by lia.
+    rewrite H0.
+    apply app_halftape_S.
+  - subst. reflexivity.
+  - subst. reflexivity.
+  - destruct x; try lia.
+    destruct (Z.pos p + -1)%Z eqn:E; try lia.
+    symmetry.
+    assert (H0:(Nat.pred (Pos.to_nat p)) = S (Nat.pred (Pos.to_nat p0))) by lia.
+    rewrite H0.
+    apply app_halftape_S.
+Qed.
+
+Definition tape_rev(f:Z->Σ):Z->Σ := fun x => f (-x)%Z.
+
+Lemma make_tape'_rev l1' l1 m1 r1 r1':
+  tape_rev (make_tape' l1' l1 m1 r1 r1') = (make_tape' r1' r1 m1 l1 l1').
+Proof.
+  fext.
+  unfold tape_rev.
+  destruct x; cbn; reflexivity.
+Qed.
+
+Lemma mov_tape_rev t d:
+  mov Σ (tape_rev t) d = tape_rev (mov Σ t (Dir_rev d)).
+Proof.
+  fext.
+  unfold mov,tape_rev.
+  f_equal.
+  destruct d; cbn; lia.
+Qed.
+
+Lemma make_tape'_mov_r l1' l1 m1 r1 r1' σ:
+  mov Σ (make_tape' l1' l1 m1 (σ :: r1) r1') Dpos = make_tape' l1' (m1 :: l1) σ r1 r1'.
+Proof.
+  rewrite <-make_tape'_rev.
+  symmetry.
+  rewrite <-make_tape'_rev.
+  rewrite mov_tape_rev.
+  cbn.
+  rewrite make_tape'_mov_l.
+  reflexivity.
+Qed.
+
+Definition half_tape_cdr(f:nat->Σ):nat->Σ :=
+  fun n => f (S n).
+
+Lemma app_halftape_cdr l1':
+  app_halftape nil l1' = app_halftape (l1' 0 :: nil) (half_tape_cdr l1').
+Proof.
+  fext.
+  destruct x; cbn.
+  1: reflexivity.
+  unfold app_halftape.
+  destruct x; reflexivity.
+Qed.
+
+Lemma app_halftape_eq_car_cdr h t t0 h' t' t0':
+  h=h' ->
+  app_halftape t t0 = app_halftape t' t0' ->
+  app_halftape (h::t) t0 = app_halftape (h'::t') t0'.
+Proof.
+  intros. subst.
+  fext.
+  destruct x.
+  - reflexivity.
+  - cbn.
+    repeat rewrite app_halftape_S.
+    cg.
+Qed.
+
+Lemma app_halftape_cdr' l0 l1':
+  app_halftape l0 l1' = app_halftape (l0 ++ l1' 0 :: nil) (half_tape_cdr l1').
+Proof.
+  induction l0.
+  - apply app_halftape_cdr.
+  - cbn.
+    apply app_halftape_eq_car_cdr; tauto.
+Qed.
+
+Lemma half_tape_cdr_cons h l1:
+  (half_tape_cdr (app_halftape (h :: nil) l1)) = l1.
+Proof.
+  unfold half_tape_cdr,app_halftape.
+  cbn.
+  fext.
+  destruct x; cbn; reflexivity.
+Qed.
+
+
+Lemma make_tape'_cdr_l l1' o r1 r1':
+  make_tape' l1' nil o r1 r1' = make_tape' (half_tape_cdr l1') (l1' 0::nil) o r1 r1'.
+Proof.
+  unfold make_tape'.
+  f_equal.
+  apply app_halftape_cdr.
+Qed.
+
+Lemma make_tape'_cdr_r l1' l1 o r1':
+  make_tape' l1' l1 o nil r1' = make_tape' l1' l1 o (r1' 0::nil) (half_tape_cdr r1').
+Proof.
+  unfold make_tape'.
+  f_equal.
+  apply app_halftape_cdr.
+Qed.
+
+Lemma app_halftape_nil l1:
+  app_halftape nil l1 = l1.
+Proof.
+  unfold app_halftape.
+  fext.
+  destruct x; cbn; reflexivity.
+Qed.
+
+Lemma make_tape'_cons_l h l1 o r1 r2:
+  (make_tape' (app_halftape (h::nil) l1) nil o r1 r2) =
+  (make_tape' l1 (h::nil) o r1 r2).
+Proof.
+  unfold make_tape'.
+  f_equal.
+  cbn.
+  rewrite app_halftape_nil.
+  reflexivity.
+Qed.
+
+Lemma make_tape'_cons_r l2 l1 o h r1:
+  (make_tape' l2 l1 o nil (app_halftape (h::nil) r1)) =
+  (make_tape' l2 l1 o (h::nil) r1).
+Proof.
+  unfold make_tape'.
+  f_equal.
+  cbn.
+  rewrite app_halftape_nil.
+  reflexivity.
+Qed.
+
+
+Lemma make_tape_eq {a b c a' b' c'}:
+  make_tape a b c = make_tape a' b' c' ->
+  (a=a'/\b=b'/\c=c').
+Proof.
+  intros.
+  repeat split.
+  - fext.
+    epose proof (fext_inv (Zneg (Pos.of_succ_nat x)) H) as H0.
+    cbn in H0.
+    rewrite SuccNat2Pos.pred_id in H0. apply H0.
+  - epose proof (fext_inv Z0 H) as H0.
+    cbn in H0. apply H0.
+  - fext.
+    epose proof (fext_inv (Zpos (Pos.of_succ_nat x)) H) as H0.
+    cbn in H0.
+    rewrite SuccNat2Pos.pred_id in H0. apply H0.
+Qed.
+
+Lemma app_halftape_eq_cons {h a b h' a' b'}:
+  app_halftape (h::a) b = app_halftape (h'::a') b' ->
+  (h=h'/\app_halftape a b = app_halftape a' b').
+Proof.
+  intro.
+  split.
+  1: apply (fext_inv 0 H).
+  fext.
+  epose proof (fext_inv (S x) H) as H0.
+  repeat rewrite app_halftape_S in H0.
+  apply H0.
+Qed.
+
+Lemma app_halftape_eq {a b a' b'}:
+  app_halftape a b = app_halftape a' b' ->
+  length a <= length a' ->
+  exists ls,
+  length ls = length a' - length a /\
+  a++ls=a' /\
+  app_halftape ls b' = b.
+Proof.
+  gd a'.
+  induction a as [|h a]; intros.
+  - exists a'. cbn.
+    repeat split.
+    1: lia.
+    rewrite <-H. apply app_halftape_nil.
+  - destruct a' as [|h' a'].
+    1: cbn in H0; lia.
+    destruct (app_halftape_eq_cons H) as [H1 H2].
+    subst.
+    cbn in H0.
+    assert (H3:length a <= length a') by lia.
+    specialize (IHa _ H2 H3).
+    destruct IHa as [ls [H4 [H5 H6]]].
+    exists ls.
+    repeat split; auto 1.
+    cbn. cg.
+Qed.
+
+Lemma app_halftape_eq' {a b a' b'}:
+  app_halftape a b = app_halftape a' b' ->
+  length a = length a' ->
+  (a=a'/\b=b').
+Proof.
+  intros.
+  eassert (H1:_) by (apply (app_halftape_eq H); lia).
+  destruct H1 as [ls [H1 [H2 H3]]].
+  assert (length ls = 0) by lia.
+  destruct ls; cbn in H4; cg.
+  rewrite app_halftape_nil in H3.
+  rewrite app_nil_r in H2.
+  split; cg.
+Qed.
+
+
+Definition AbstractSteps tm n0 (st0 st1:ListES) :=
+  length st0.(l) + length st0.(r) = length st1.(l) + length st1.(r) /\
+  forall l1 r1,
+    Steps Σ tm n0 (makeES st0 l1 r1) (makeES st1 l1 r1).
+
+Fixpoint getASteps(h:St*Σ*(Trans Σ))(ls:list (St*Σ*(Trans Σ))):ListES*ListES :=
+  match h with
+  | (s'',i'',tr'') =>
+    match ls with
+    | nil =>
+      let x:=Build_ListES nil nil i'' s'' in
+      (x,x)
+    | h0::t0 =>
+      let (st0,st1):=getASteps h0 t0 in
+      let (l0,r0,m0,s0):=st0 in
+      let (l1,r1,m1,s1):=st1 in
+      match h0 with
+      | (s',i',tr') =>
+        let (s_,d,o):=tr' in
+        match d with
+        | Dpos =>
+          match r1 with
+          | nil =>
+            (Build_ListES l0 (r0++i''::nil) m0 s0,
+             Build_ListES (o::l1) nil i'' s'')
+          | m2::r2 =>
+            (st0, Build_ListES (o::l1) r2 m2 s'')
+          end
+        | Dneg =>
+          match l1 with
+          | nil =>
+            (Build_ListES (l0++i''::nil) r0 m0 s0,
+             Build_ListES nil (o::r1) i'' s'')
+          | m2::l2 =>
+            (st0, Build_ListES l2 (o::r1) m2 s'')
+          end
+        end
+      end
+    end
+  end.
+
+(* gen unique Asteps from (St,Σ) history *)
+
+
+Inductive MoveDist: (TM Σ)->(nat)->(ExecState Σ)->(ExecState Σ)->Z->Prop :=
+| MoveDist_O tm st: MoveDist tm O st st Z0
+| MoveDist_S tm n st0 s1 t1 st2 d d' tr:
+  MoveDist tm n st0 (s1,t1) d ->
+  step Σ tm (s1,t1) = Some st2 ->
+  tm s1 (t1 Z0) = Some tr ->
+  (d'-d = (Dir_to_Z (dir _ tr)))%Z ->
+  MoveDist tm (S n) st0 st2 d'
+.
+
+Lemma MoveDist_unique {tm n st0 st1 d st1' d'}:
+  MoveDist tm n st0 st1 d ->
+  MoveDist tm n st0 st1' d' ->
+  (st1=st1' /\ d=d').
+Proof.
+  gd d'. gd st1'.
+  gd d. gd st1.
+  induction n.
+  - intros.
+    invst H. invst H0. tauto.
+  - intros.
+    invst H. invst H0.
+    specialize (IHn _ _ _ _ H2 H5).
+    destruct IHn as [IHn0 IHn1].
+    invst IHn0.
+    rewrite H8 in H4.
+    invst H4.
+    rewrite H7 in H3.
+    invst H3.
+    repeat split.
+    rewrite <-H10 in H6.
+    lia.
+Qed.
+
+Lemma getASteps_spec {tm:TM Σ} {n st0 st1 h ls}:
+  Steps _ tm n st0 st1 ->
+  length ls = n ->
+  (forall n0, n0<=n -> exists s2 t2, Steps _ tm n0 st0 (s2,t2) /\
+  match nth_error (h::ls) (n-n0) with
+  | None => False
+  | Some (s0,i0,tr) => tm s0 i0 = Some tr /\ s0 = s2 /\ i0 = t2 Z0
+  end) ->
+  let (st0',st1'):=getASteps h ls in
+  AbstractSteps tm n st0' st1' /\
+  (MoveDist tm n st0 st1 ((Z.of_nat (length (st1'.(l))))-(Z.of_nat (length (st0'.(l)))))) /\
+  exists l1 r1,
+  st0 = makeES st0' l1 r1 /\
+  st1 = makeES st1' l1 r1.
+Proof.
+  gd st1.
+  gd h. gd ls.
+  induction n; intros.
+  - destruct ls.
+    2: cbn in H0; cg.
+    specialize (H1 0).
+    assert (H2:0<=0) by lia.
+    specialize (H1 H2). clear H2.
+    cbn in H1.
+    destruct H1 as [s2 [t2 [H1a H1b]]].
+    destruct h as [[s0 i0] tr].
+    destruct H1b as [H1b [H1c H1d]]. subst.
+    cbn.
+    epose proof (Steps_unique _ H1a H). subst.
+    invst H1a.
+    split.
+    {
+      split.
+      1: cg.
+      intros. ctor.
+    }
+    split.
+    1: ctor.
+    eexists. eexists.
+    rewrite <-make_tape'_lmr.
+    tauto.
+  - destruct ls as [|h0 ls]; cbn in H0.
+    1: cg.
+    invst H.
+    invst H0.
+    specialize (IHn ls h0 _ H3 eq_refl).
+    cbn.
+    destruct (getASteps h0 ls) as [st3 st4].
+    eassert (H':_). {
+      apply IHn.
+      intros.
+      specialize (H1 n0).
+      assert (H4:S (length ls) - n0 = S ((length ls) - n0)) by lia.
+      rewrite H4 in H1.
+      cbn in H1.
+      apply H1. lia.
+    }
+    clear IHn.
+    destruct H' as [H'AS [H'md [l1' [r1' [H'0 H'1]]]]].
+    destruct h as [[s'' i''] tr''].
+    destruct h0 as [[s' i'] tr'].
+    destruct st3 as [l0 r0 m0 s0].
+    destruct st4 as [l1 r1 m1 s1].
+    eassert (H1a:_) by (apply (H1 (length ls)); lia).
+    eassert (H1b:_) by (apply (H1 (S (length ls))); lia).
+    clear H1.
+    destruct H1a as [s2a [t2a [H1a1 H1a2]]].
+    destruct H1b as [s2b [t2b [H1b1 H1b2]]].
+    epose proof (Steps_unique _ H1a1 H3) as H1.
+    epose proof (Steps_unique _ H1b1 H) as H2.
+    destruct st2 as [s2 t2].
+    destruct st1 as [s1' t1].
+    invst H1.
+    invst H2.
+    clear H1a1. clear H1b1.
+    clear H1. clear H2.
+    assert (H1:S (length ls) - length ls = 1) by lia.
+    rewrite H1 in H1a2. clear H1.
+    rewrite Nat.sub_diag in H1b2.
+    cbn in H1a2,H1b2.
+    destruct H1a2 as [H1a1 [H1a2 H1a3]].
+    destruct H1b2 as [H1b1 [H1b2 H1b3]].
+    subst.
+    destruct tr' as [s' d o].
+    destruct d.
+    {
+      destruct l1.
+      - split.
+        {
+          destruct H'AS as [H'len H'AS].
+          split.
+          1: cbn; cbn in H'len; rewrite app_length; cbn; lia.
+          intros.
+          pose proof (H'AS (app_halftape (t1 Z0::nil) l1) r2) as H1.
+          ector.
+          - assert (E2:(makeES {| l := l0; r := r0; m := m0; s := s0 |} (app_halftape (t1 0%Z :: nil) l1) r2) = 
+            (makeES {| l := l0 ++ t1 0%Z :: nil; r := r0; m := m0; s := s0 |} l1 r2)). {
+              cbn. f_equal. unfold make_tape'. f_equal.
+              rewrite app_halftape_cdr'.
+              rewrite half_tape_cdr_cons.
+              cbn.
+              reflexivity.
+            }
+            rewrite E2 in H1.
+            apply H1.
+          - cbn.
+            cbn in H'1.
+            invst H'1.
+            cbn in H1a1.
+            rewrite H1a1.
+            cbn in H5.
+            rewrite H1a1 in H5.
+            inversion H5.
+            repeat rewrite H6.
+            f_equal.
+            f_equal.
+            rewrite make_tape'_upd.
+            rewrite make_tape'_cons_l.
+            rewrite make_tape'_mov_l.
+            reflexivity.
+        }
+        split.
+        {
+          cbn.
+          cbn in H'md.
+          ector; eauto 1.
+          cbn.
+          rewrite app_length.
+          cbn. lia.
+        }
+        exists (half_tape_cdr l1').
+        exists r1'.
+        split.
+        + cbn. f_equal.
+          unfold make_tape'.
+          f_equal.
+          assert (t1 Z0 = l1' 0). {
+            cbn in H'1.
+            inversion H'1.
+            subst.
+            cbn in H5.
+            cbn in H1a1.
+            rewrite H1a1 in H5.
+            invst H5. clear H5.
+            rewrite make_tape'_upd.
+            rewrite make_tape'_cdr_l.
+            rewrite make_tape'_mov_l.
+            reflexivity.
+          }
+          rewrite H1.
+          apply app_halftape_cdr'.
+        + cbn.
+          f_equal.
+          cbn in H5.
+          rewrite H1a1 in H5.
+          inversion H5.
+          cbn in H'1.
+          inversion H'1.
+          rewrite make_tape'_upd.
+
+          repeat rewrite make_tape'_cdr_l.
+          rewrite make_tape'_mov_l.
+          rewrite make_tape'_cdr_l.
+          reflexivity.
+      - split.
+        {
+          destruct H'AS as [H'len H'AS].
+          split.
+          1: cbn; cbn in H'len; lia.
+          intros.
+          ector; eauto 1.
+          cbn.
+          cbn in H'1.
+          invst H'1.
+          cbn in H1a1.
+          rewrite H1a1.
+          cbn in H5.
+          rewrite H1a1 in H5.
+          invst H5.
+          rewrite make_tape'_upd.
+          rewrite make_tape'_mov_l.
+          reflexivity.
+        }
+        clear H'AS.
+        split.
+        {
+          cbn.
+          cbn in H'md.
+          ector; eauto 1.
+          cbn.
+          destruct (Z.of_nat (length l0))%Z eqn:E; cbn; try lia.
+          rewrite <-Pos2Z.add_pos_neg.
+          lia.
+        }
+        clear H'md.
+        exists l1'. exists r1'.
+        split. 1: reflexivity.
+        cbn. f_equal.
+        cbn in H'1.
+        inversion H'1. clear H'1.
+        clear H2. clear s1.
+        cbn in H5.
+        rewrite H1a1 in H5.
+        invst H5.
+        inversion H5. clear H5.
+        rewrite make_tape'_upd,make_tape'_mov_l.
+        reflexivity.
+    }
+    {
+      destruct r1.
+      - split.
+        {
+          destruct H'AS as [H'len H'AS].
+          split.
+          1: cbn; cbn in H'len; rewrite app_length; cbn; lia.
+          intros.
+          pose proof (H'AS l2 (app_halftape (t1 Z0::nil) r1)) as H1.
+          ector.
+          - assert (E2:
+              (makeES {| l := l0; r := r0; m := m0; s := s0 |} l2 (app_halftape (t1 0%Z :: nil) r1)) =
+              (makeES {| l := l0; r := r0 ++ t1 0%Z :: nil; m := m0; s := s0 |} l2 r1)
+            ). {
+              cbn. f_equal. unfold make_tape'. f_equal.
+              rewrite app_halftape_cdr'.
+              rewrite half_tape_cdr_cons.
+              cbn.
+              reflexivity.
+            }
+            rewrite E2 in H1.
+            apply H1.
+          - cbn.
+            cbn in H'1.
+            invst H'1.
+            cbn in H1a1.
+            rewrite H1a1.
+            cbn in H5.
+            rewrite H1a1 in H5.
+            inversion H5.
+            repeat rewrite H6.
+            f_equal.
+            f_equal.
+            rewrite make_tape'_upd.
+            rewrite make_tape'_cons_r.
+            rewrite make_tape'_mov_r.
+            reflexivity.
+        }
+        split.
+        {
+          cbn.
+          cbn in H'md.
+          ector; eauto 1.
+          cbn.
+          destruct (Z.of_nat (length l0)) eqn:E; cbn; (repeat rewrite <-Pos2Z.add_pos_neg); try lia.
+          destruct ((Z.of_nat (length l1) - 0) %Z) eqn:E0; cbn; (repeat rewrite <-Pos2Z.add_pos_neg); try lia.
+        }
+        exists l1'.
+        exists (half_tape_cdr r1').
+        split.
+        + cbn. f_equal.
+          unfold make_tape'.
+          f_equal.
+          assert (t1 Z0 = r1' 0). {
+            cbn in H'1.
+            inversion H'1.
+            subst.
+            cbn in H5.
+            cbn in H1a1.
+            rewrite H1a1 in H5.
+            invst H5. clear H5.
+            rewrite make_tape'_upd.
+            rewrite make_tape'_cdr_r.
+            rewrite make_tape'_mov_r.
+            reflexivity.
+          }
+          rewrite H1.
+          apply app_halftape_cdr'.
+        + cbn.
+          f_equal.
+          cbn in H5.
+          rewrite H1a1 in H5.
+          inversion H5.
+          cbn in H'1.
+          inversion H'1.
+          rewrite make_tape'_upd.
+
+          repeat rewrite make_tape'_cdr_r.
+          rewrite make_tape'_mov_r.
+          rewrite make_tape'_cdr_r.
+          reflexivity.
+      - split.
+        {
+          destruct H'AS as [H'len H'AS].
+          split.
+          1: cbn; cbn in H'len; lia.
+          intros.
+          ector; eauto 1.
+          cbn.
+          cbn in H'1.
+          invst H'1.
+          cbn in H1a1.
+          rewrite H1a1.
+          cbn in H5.
+          rewrite H1a1 in H5.
+          invst H5.
+          rewrite make_tape'_upd.
+          rewrite make_tape'_mov_r.
+          reflexivity.
+        }
+        clear H'AS.
+        split.
+        {
+          cbn.
+          cbn in H'md.
+          ector; eauto 1.
+          cbn.
+          destruct (Z.of_nat (length l0))%Z eqn:E; cbn; try lia.
+          destruct ((Z.of_nat (length l1) - 0) %Z) eqn:E0; cbn; (repeat rewrite <-Pos2Z.add_pos_neg); try lia.
+          rewrite <-Pos2Z.add_pos_neg. lia.
+        }
+        clear H'md.
+        exists l1'. exists r1'.
+        split. 1: reflexivity.
+        cbn. f_equal.
+        cbn in H'1.
+        inversion H'1. clear H'1.
+        clear H2. clear s1.
+        cbn in H5.
+        rewrite H1a1 in H5.
+        invst H5.
+        inversion H5. clear H5.
+        rewrite make_tape'_upd,make_tape'_mov_r.
+        reflexivity.
+    }
+Qed.
+
+
+Lemma ex_sitr_history {tm:TM Σ} {n st0 st1}:
+  Steps _ tm (S n) st0 st1 ->
+  exists h ls,
+  length ls = n /\
+  (forall n0, n0<=n -> exists s2 t2, Steps _ tm n0 st0 (s2,t2) /\
+  match nth_error (h::ls) (n-n0) with
+  | None => False
+  | Some (s0,i0,tr) => tm s0 i0 = Some tr /\ s0 = s2 /\ i0 = t2 Z0
+  end).
+Proof.
+  gd st1.
+  induction n.
+  - intros.
+    invst H.
+    invst H1. clear H. clear H1.
+    destruct st2 as [s0 t0].
+    cbn in H3.
+    destruct (tm s0 (t0 Z0)) as [tr|] eqn:E. 2: cg.
+    exists (s0,t0 Z0,tr).
+    exists nil.
+    cbn.
+    split. 1: reflexivity.
+    intros.
+    destruct n0. 2: lia.
+    exists s0. exists t0.
+    split.
+    1: ctor.
+    repeat split.
+    cg.
+  - intros.
+    invst H.
+    specialize (IHn _ H1).
+    destruct IHn as [h' [ls' [IHn1 IHn2]]].
+    destruct st2 as [s0 t0].
+    cbn in H3.
+    destruct (tm s0 (t0 Z0)) as [tr|] eqn:E. 2: cg.
+    exists (s0,t0 Z0,tr).
+    exists (h'::ls').
+    split.
+    1: cbn; cg.
+    intros.
+    assert (H2:n0<=n\/n0=S n) by lia.
+    destruct H2 as [H2|H2].
+    + assert (H4:S n - n0 = S (n-n0)) by lia.
+      rewrite H4. cbn.
+      apply IHn2,H2.
+    + assert (H4:S n - n0 = 0) by lia.
+      rewrite H4. cbn.
+      subst.
+      exists s0. exists t0.
+      split; tauto.
+Qed.
+
+Lemma Steps_split{tm n1 n2 st0 st1}:
+  Steps Σ tm (n1+n2) st0 st1 ->
+  exists st2,
+  Steps Σ tm n2 st0 st2 /\
+  Steps Σ tm n1 st2 st1.
+Proof.
+  gd st1.
+  induction n1; intros.
+  - exists st1.
+    split. 1: apply H.
+    ctor.
+  - invst H.
+    specialize (IHn1 _ H1).
+    destruct IHn1 as [st3 [I1 I2]].
+    exists st3.
+    split; auto 1.
+    ector; eauto 1.
+Qed.
+
+Lemma half_tape_make_tape_r {l0 m0 r0}:
+  (half_tape (make_tape l0 m0 r0)) 1 Dpos = r0.
+Proof.
+  unfold make_tape,half_tape,addmul,Dir_to_Z.
+  fext.
+  destruct (1 + 1 * Z.of_nat x)%Z eqn:E; try lia.
+  f_equal.
+  lia.
+Qed.
+
+Lemma half_tape_make_tape_l {l0 m0 r0}:
+  (half_tape (make_tape l0 m0 r0)) (-1) Dneg = l0.
+Proof.
+  unfold make_tape,half_tape,addmul,Dir_to_Z.
+  fext.
+  destruct (-1 + -1 * Z.of_nat x)%Z eqn:E; try lia.
+  f_equal.
+  lia.
+Qed.
+
+Definition half_tape_all0:nat->Σ :=
+  (fun _=>Σ0).
+
+Lemma app_halftape_all0{l1 l2}:
+  app_halftape l1 l2 = half_tape_all0 ->
+  l2 = half_tape_all0.
+Proof.
+  unfold half_tape_all0.
+  intros.
+  fext.
+  epose proof (fext_inv ((length l1)+x) H) as H0.
+  cbn in H0.
+  unfold app_halftape in H0.
+  destruct (nth_error l1 (length l1 + x)) eqn:E.
+  - assert (E1:length l1 <= length l1 + x) by lia.
+    rewrite <-nth_error_None in E1. cg.
+  - rewrite <-H0. f_equal. lia.
+Qed.
+
+Lemma app_halftape_assoc{l1 l2 l3}:
+  app_halftape l1 (app_halftape l2 l3) =
+  app_halftape (l1++l2) l3.
+Proof.
+  induction l1.
+  - cbn. rewrite app_halftape_nil. reflexivity.
+  - cbn. apply app_halftape_eq_car_cdr; auto 1.
+Qed.
+
+
+Lemma loop1_nonhalt (tm:TM Σ) n s0 t0:
+  n<>0 ->
+  (forall n0, n0<=n -> exists s2 t2 s2' t2',
+    Steps _ tm n0 (s0,t0) (s2,t2) /\
+    Steps _ tm (n+n0) (s0,t0) (s2',t2') /\
+    s2=s2' /\
+    t2 Z0 = t2' Z0) ->
+  (exists s2 t2 d, MoveDist tm n (s0,t0) (s2,t2) d /\
+    (d=Z0 \/
+    (d>0)%Z /\
+    ((half_tape t0 1 Dpos)=half_tape_all0)
+    \/
+    (d<0)%Z /\
+    ((half_tape t0 (-1) Dneg)=half_tape_all0)
+  )) ->
+  ~Halts _ tm (s0,t0).
+Proof.
+  intros.
+  assert (exists st0, Steps _ tm (S(n+n)) (s0,t0) st0). {
+    eassert (H2:_) by (apply (H0 n); lia).
+    eassert (H3:_) by (apply (H0 1); lia).
+    destruct H2 as [s20 [t20 [s2'0 [t2'0 [H21 [H22 [H23 H24]]]]]]].
+    destruct H3 as [s21 [t21 [s2'1 [t2'1 [H31 [H32 [H33 H34]]]]]]].
+    subst.
+    rewrite Nat.add_1_r in H32.
+    inversion H32.
+    epose proof (Steps_unique _ H21 H3). subst.
+    cbn in H5.
+    rewrite H24 in H5.
+    destruct (tm s2'0 (t2'0 0%Z)) as [tr|] eqn:E; cg.
+    destruct tr as [s' d o].
+    eexists.
+    ector.
+    1: apply H22.
+    cbn.
+    rewrite E.
+    reflexivity.
+  }
+  destruct H2 as [st2 H2].
+  assert (E1:S (n+n) = (S n)+n) by lia.
+  rewrite E1 in H2.
+  epose proof (Steps_split H2) as H3.
+  destruct H3 as [st3 [H3 H4]].
+  epose proof (ex_sitr_history H4) as H5.
+  destruct H5 as [h [ls [H5a H5b]]].
+  inversion H4.
+  epose proof (getASteps_spec H6 H5a H5b) as X1. subst.
+
+  rewrite Nat.add_comm in H2.
+  epose proof (Steps_split H2) as H3'.
+  destruct H3' as [st3' [H3' H4']].
+  epose proof (ex_sitr_history H3') as H5'.
+  destruct H5' as [h' [ls' [H5a' H5b']]].
+  inversion H3'.
+  epose proof (getASteps_spec H7 H5a' H5b') as X2. subst.
+
+  assert (E2:(h'::ls')=(h::ls)). {
+    apply list_eq__nth_error.
+    1: cbn; cg.
+    intros n H5. cbn in H5.
+    eassert (A:_) by (apply (H5b (length ls - n)); lia).
+    eassert (A':_) by (apply (H5b' (length ls' - n)); lia).
+    assert (B1:(length ls - (length ls - n)) = n) by lia.
+    assert (B1':(length ls - (length ls' - n)) = n) by lia.
+    rewrite B1 in A. clear B1.
+    rewrite B1' in A'. clear B1'.
+    destruct A as [s2 [t2 [A1 A2]]].
+    destruct A' as [s2' [t2' [A1' A2']]].
+    destruct (nth_error (h :: ls) n). 2: contradiction.
+    destruct (nth_error (h' :: ls') n). 2: contradiction.
+    destruct p as [[s4 i4] tr].
+    destruct p0 as [[s4' i4'] tr'].
+    destruct A2 as [A2 [A3 A4]].
+    destruct A2' as [A2' [A3' A4']].
+    subst.
+    epose proof (Steps_trans _ H3 A1) as B1.
+    eassert (B2:_) by (apply (H0 (length ls - n)); lia).
+    rewrite H5a' in A1'.
+    destruct B2 as [s5 [i5 [s6 [i6 [B2 [B3 [B4 B5]]]]]]].
+    rewrite Nat.add_comm in B3.
+    epose proof (Steps_unique _ B3 B1) as B6.
+    epose proof (Steps_unique _ A1' B2) as B7.
+    invst B6. invst B7.
+    rewrite B5.
+    rewrite B5 in A2'.
+    rewrite A2' in A2.
+    invst A2.
+    reflexivity.
+  }
+  invst E2. clear E2.
+  destruct (getASteps h ls) as [st0' st1'].
+  epose proof (Steps_unique _ H3 H7); subst.
+  destruct X1 as [X1a [X1b [l1 [r1 [X1c X1d]]]]].
+  destruct X2 as [X2a [X2b [l1' [r1' [X2c X2d]]]]].
+  destruct st1 as [s1 t1].
+  destruct st0 as [s2 t2].
+  destruct st0' as [l'0 r'0 m'0 s'0].
+  destruct st1' as [l'1 r'1 m'1 s'1].
+  cbn in X1c,X1d,X2c,X2d.
+  inversion X1c.
+  inversion X1d.
+  inversion X2c.
+  inversion X2d.
+  subst s'0. subst s'1. subst s1. subst s2.
+  clear X1c. clear X1d.
+  clear X2c. clear X2d.
+  cbn in X1b,X2b.
+  assert (m'0=m'1). {
+    rewrite H17 in H11.
+    pose proof (fext_inv Z0 H11).
+    cbn in H5. cg.
+  }
+  subst m'1.
+  destruct X2a as [X3 X4].
+  cbn in X3.
+
+  destruct H1 as [s7 [t7 [d [H1a H1b]]]].
+  epose proof (MoveDist_unique H1a X2b) as C1.
+  destruct C1 as [C1 C2].
+  inversion C1. subst s7. subst t7. clear C1.
+
+  rewrite H11 in H17.
+  destruct (make_tape_eq H17) as [D1 [D2 D3]].
+
+
+  destruct H1b as [H1b|[H1b|H1b]].
+  {
+    subst d.
+    assert (E2:length l'1 = length l'0) by lia.
+    assert (E3:length r'1 = length r'0) by lia.
+    symmetry in E2,E3.
+    destruct (app_halftape_eq' D1 E2) as [D1a D1b].
+    destruct (app_halftape_eq' D3 E3) as [D2a D2b].
+    subst.
+    intro F1.
+    destruct F1 as [n F1].
+    remember (s0, make_tape' l1' l'1 m'0 r'1 r1') as st.
+    remember (length ls) as n0.
+    assert (G1:forall n2, Steps _ tm (n2*n0) st st). {
+      intros.
+      induction n2.
+      - cbn. ctor.
+      - cbn. eapply Steps_trans; eauto 1.
+    }
+    specialize (G1 (S n)).
+    destruct n0 as [|n0]. 1: lia.
+    eapply (Steps_NonHalt); eauto 1. lia.
+  }
+  {
+    destruct H1b as [H1b H1c].
+    subst d.
+    assert (E2:length l'0 <= length l'1) by lia.
+    assert (E3:length r'1 <= length r'0) by lia.
+    destruct (app_halftape_eq D1 E2) as [l3 [D1a [D1b D1c]]].
+    symmetry in D3.
+    destruct (app_halftape_eq D3 E3) as [r3 [D2a [D2b D2c]]].
+    subst.
+    clear D1. clear D2. clear D3.
+    unfold make_tape' in H1c.
+    rewrite half_tape_make_tape_r in H1c.
+
+
+    unfold makeES in X4.
+    remember (length ls) as n0.
+    assert (G1:forall n2, exists l5, Steps _ tm (n2*n0)
+    (s0, make_tape' l1' l'0 m'0 (r'1 ++ r3) (app_halftape r3 r1))
+    (s0, make_tape' l1' (l'0++l5) m'0 (r'1 ++ r3) (app_halftape r3 r1))
+    ). {
+      intros.
+      induction n2.
+      1: exists nil; cbn; rewrite app_nil_r; ctor.
+      destruct IHn2 as [l5 IHn2].
+      exists (l3++l5).
+      cbn.
+      eapply Steps_trans; eauto 1.
+      epose proof (X4 (app_halftape l5 l1') (app_halftape r3 r1)) as G2.
+      unfold make_tape' in G2.
+      unfold make_tape'.
+
+      repeat rewrite app_halftape_assoc in G2.
+      repeat rewrite <-app_assoc in G2.
+      repeat rewrite app_halftape_assoc.
+      repeat rewrite <-app_assoc.
+
+      pose proof (app_halftape_all0 H1c) as E4.
+      pose proof (app_halftape_all0 E4) as E5.
+
+      pose proof H1c as H1d.
+      rewrite E4,<-E5 in H1d.
+      repeat rewrite app_halftape_assoc in H1c.
+      repeat rewrite <-app_assoc in H1c.
+      rewrite H1c.
+      rewrite H1c in G2.
+      rewrite H1d,E5 in G2.
+      apply G2.
+    }
+    intro F1.
+    destruct F1 as [n F1].
+    specialize (G1 (S n)).
+    destruct G1 as [l5 G1].
+    destruct n0 as [|n0]. 1: lia.
+    eapply (Steps_NonHalt); eauto 1. lia.
+  }
+  {
+    destruct H1b as [H1b H1c].
+    subst d.
+    assert (E2:length l'1 <= length l'0) by lia.
+    assert (E3:length r'0 <= length r'1) by lia.
+    symmetry in D1.
+    destruct (app_halftape_eq D1 E2) as [l3 [D1a [D1b D1c]]].
+    destruct (app_halftape_eq D3 E3) as [r3 [D2a [D2b D2c]]].
+    subst.
+    clear D1. clear D2. clear D3.
+    unfold make_tape' in H1c.
+    rewrite half_tape_make_tape_l in H1c.
+
+
+    unfold makeES in X4.
+    remember (length ls) as n0.
+    assert (G1:forall n2, exists r5, Steps _ tm (n2*n0)
+      (s0, make_tape' (app_halftape l3 l1) (l'1 ++ l3) m'0 r'0 r1')
+      (s0, make_tape' (app_halftape l3 l1) (l'1 ++ l3) m'0 (r'0++r5) r1')
+    ). {
+      intros.
+      induction n2.
+      1: exists nil; cbn; rewrite app_nil_r; ctor.
+      destruct IHn2 as [r5 IHn2].
+      exists (r3++r5).
+      cbn.
+      eapply Steps_trans; eauto 1.
+      epose proof (X4 (app_halftape l3 l1) (app_halftape r5 r1')) as G2.
+      unfold make_tape' in G2.
+      unfold make_tape'.
+
+      repeat rewrite app_halftape_assoc in G2.
+      repeat rewrite <-app_assoc in G2.
+      repeat rewrite app_halftape_assoc.
+      repeat rewrite <-app_assoc.
+
+      pose proof (app_halftape_all0 H1c) as E4.
+      pose proof (app_halftape_all0 E4) as E5.
+
+      pose proof H1c as H1d.
+      rewrite E4,<-E5 in H1d.
+      repeat rewrite app_halftape_assoc in H1c.
+      repeat rewrite <-app_assoc in H1c.
+      rewrite H1c.
+      rewrite H1c in G2.
+      rewrite H1d,E5 in G2.
+      apply G2.
+    }
+    intro F1.
+    destruct F1 as [n F1].
+    specialize (G1 (S n)).
+    destruct G1 as [l5 G1].
+    destruct n0 as [|n0]. 1: lia.
+    eapply (Steps_NonHalt); eauto 1. lia.
+  }
+Qed.
+
+
+Definition ListES_step'(tr:Trans Σ)(x:ListES):ListES :=
+let (l0,r0,m0,s0):=x in
+  let (s1,d,o) := tr in
+    match d with
+    | Dpos =>
+      match r0 with
+      | m1::r1 => {| l:=o::l0; r:=r1; m:=m1; s:=s1 |}
+      | nil => {| l:=o::l0; r:=nil; m:=Σ0; s:=s1 |}
+      end
+    | Dneg =>
+      match l0 with
+      | m1::l1 => {| l:=l1; r:=o::r0; m:=m1; s:=s1 |}
+      | nil => {| l:=nil; r:=o::r0; m:=Σ0; s:=s1 |}
+      end
+    end.
+
+Lemma ListES_step'_spec tm l0 r0 m0 s0:
+  step Σ tm (ListES_toES (Build_ListES l0 r0 m0 s0)) =
+  match tm s0 m0 with
+  | Some tr => Some (ListES_toES (ListES_step' tr (Build_ListES l0 r0 m0 s0)))
+  | None => None
+  end.
+Proof.
+  erewrite (ListES_step_spec).
+  cbn.
+  destruct (tm s0 m0) as [[s1 d o]|]; reflexivity.
+Qed.
+
+Fixpoint verify_loop1(h0 h1:ListES*Z)(ls0 ls1:list (ListES*Z))(n:nat)(dpos:Z):bool :=
+  let (es0,d0):=h0 in
+  let (es1,d1):=h1 in
+  St_eqb es0.(s) es1.(s) &&&
+  Σ_eqb es0.(m) es1.(m) &&&
+  (
+    match n with
+    | O =>
+      match dpos with
+      | Z0 => Z.eqb d1 d0
+      | Zpos _ =>
+        match es1.(r) with
+        | nil => Z.ltb d1 d0
+        | _ => false
+        end
+      | Zneg _ =>
+        match es1.(l) with
+        | nil => Z.ltb d0 d1
+        | _ => false
+        end
+      end
+    | _ => false
+    end |||
+    match ls0,ls1 with
+    | h0'::ls0',h1'::ls1' =>
+      verify_loop1 h0' h1' ls0' ls1' (Nat.pred n) dpos
+    | _,_ => false
+    end
+  ).
+
+
+
+Fixpoint find_loop1(h0 h1 h2:ListES*Z)(ls0 ls1 ls2:list (ListES*Z))(n:nat){struct ls1}:bool :=
+(
+  (let (es0,d0):=h0 in
+  let (es1,d1):=h1 in
+  St_eqb es0.(s) es1.(s) &&&
+  let (es2,d2):=h2 in
+  St_eqb es0.(s) es2.(s) &&&
+
+  Σ_eqb es0.(m) es1.(m) &&&
+  Σ_eqb es0.(m) es2.(m) &&&
+
+  (verify_loop1 h0 h1 ls0 ls1 (S n) (d0-d1)))
+)|||
+  match ls2,ls1 with
+  | h3::h2'::ls2',h1'::ls1' =>
+    find_loop1 h0 h1' h2' ls0 ls1' ls2' (S n)
+  | _,_ => false
+  end.
+
+Definition find_loop1_0(h0 h1:ListES*Z)(ls:list (ListES*Z)):bool :=
+match ls with
+| h2::ls' => find_loop1 h0 h1 h2 (h1::ls) ls ls' O
+| nil => false
+end.
+
+Definition sidpos_history_WF tm (h:ListES*Z)(ls:list (ListES*Z)):=
+  forall n, n<=(length ls) ->
+  match nth_error (h::ls) ((length ls)-n) with
+  | Some (es,d) => MoveDist tm n (InitES Σ Σ0) (ListES_toES es) d
+  | None => False
+  end.
+
+Definition sidpos_history_period (h:ListES*Z)(ls:list (ListES*Z))(n1 T:nat):=
+  forall n, n<n1 ->
+  match nth_error (h::ls) n,nth_error (h::ls) (T+n) with
+  | Some (es1,d1),Some (es2,d2) => es1.(s) = es2.(s) /\ es1.(m) = es2.(m)
+  | _,_ => False
+  end.
+
+Lemma sidpos_history_WF_cdr tm h h1 ls:
+  sidpos_history_WF tm h (h1::ls) ->
+  sidpos_history_WF tm h1 ls.
+Proof.
+  unfold sidpos_history_WF.
+  intros.
+  specialize (H n).
+  replace (length (h1 :: ls) - n) with (S (length ls - n)) in H.
+  apply H.
+  cbn. lia.
+  cbn. destruct n; lia.
+Qed.
+
+Lemma skipn_S {T} {n} {h:T} {t ls}:
+  h::t = skipn n ls ->
+  t = skipn (S n) ls.
+Proof.
+  gd ls. gd t. gd h.
+  induction n; intros.
+  - cbn. cbn in H.
+    subst. reflexivity.
+  - destruct ls as [|h0 t0].
+    1: cbn in H; cg.
+    cbn in H. cbn.
+    apply (IHn _ _ _ H).
+Qed.
+
+Lemma skipn_S' {T} {n} {h h':T} {t t'}:
+  h::t = skipn n (h'::t') ->
+  t = skipn n t'.
+Proof.
+gd t. gd t'. gd h. gd h'.
+induction n; intros.
+- cbn. invst H. reflexivity.
+- destruct t' as [|h'' t''].
+  1: cbn in H; rewrite skipn_nil in H; invst H.
+  cbn. cbn in H.
+  eapply IHn; eauto 1.
+Qed.
+
+Lemma nth_error_skipn {T} {h:T} {ls0 ls1 n}:
+  h :: ls1 = skipn n ls0 ->
+  nth_error ls0 n = Some h.
+Proof.
+  gd ls1. gd ls0. gd h.
+  induction n; intros.
+  - cbn. cbn in H.
+    rewrite <-H. reflexivity.
+  - cbn. destruct ls0 as [|h1 ls0].
+    1: invst H.
+    cbn in H.
+    eapply IHn; eauto 1.
+Qed.
+
+Lemma skipn_S_n {T} n (ls:list T):
+  skipn (S n) ls = tl (skipn n ls).
+Proof.
+  gd ls.
+  induction n; intros.
+  1: reflexivity.
+  cbn.
+  destruct ls.
+  1: reflexivity.
+  destruct ls.
+  1: rewrite skipn_nil; reflexivity.
+  specialize (IHn (t0::ls)).
+  rewrite <-IHn.
+  reflexivity.
+Qed.
+
+Lemma skipn_skipn {T} n1 n2 (ls:list T):
+  skipn n1 (skipn n2 ls) = skipn (n1+n2) ls.
+Proof.
+  gd ls. gd n2.
+  induction n1; intros.
+  1: reflexivity.
+  epose proof (IHn1 n2 ls).
+  assert (E:S n1 + n2 = S (n1+n2)) by lia.
+  rewrite E.
+  repeat rewrite skipn_S_n.
+  f_equal. apply IHn1.
+Qed.
+
+
+
+Lemma sidpos_history_period_S {h0 ls0 ls1 ls2 l0 l1 z z0 N T}:
+  (l0, z) :: ls1 = skipn N (h0 :: ls0) ->
+  (l1, z0) :: ls2 = skipn (S T) ((l0, z) :: ls1) ->
+  sidpos_history_period h0 ls0 N (S T) ->
+  s l0 = s l1 ->
+  m l0 = m l1 ->
+  sidpos_history_period h0 ls0 (S N) (S T).
+Proof.
+  unfold sidpos_history_period. cbn.
+  intros.
+  assert (E1:n<N\/n=N) by lia.
+  destruct E1 as [E1|E1].
+  1: apply H1,E1.
+  subst.
+  erewrite nth_error_skipn; eauto 1. cbn.
+  assert (H5:(l1, z0) :: ls2 = skipn (S T) ((l0,z)::ls1)) by apply H0. clear H0.
+  rewrite H in H5.
+  rewrite skipn_skipn in H5. cbn in H5.
+  erewrite nth_error_skipn; eauto 1. cbn.
+  split; auto 1.
+Qed.
+
+Lemma sidpos_history_period_S' {h0 h0' ls0' N T}:
+  sidpos_history_period h0 (h0' :: ls0') (S N) (S T) ->
+  sidpos_history_period h0' ls0' N (S T).
+Proof.
+  unfold sidpos_history_period.
+  intros.
+  specialize (H (S n)).
+  replace (S T + S n) with (S (S T + n)) in H by lia.
+  cbn in H. cbn.
+  apply H. lia.
+Qed.
+
+Lemma Steps_NonHalt_trans {tm n st st0}:
+  Steps Σ tm n st st0 ->
+  ~Halts Σ tm st0 ->
+  ~Halts Σ tm st.
+Proof.
+  repeat rewrite <-NonHalt_iff.
+  unfold NonHalt.
+  intros.
+  assert (E:n0<n\/n<=n0) by lia.
+  destruct E as [E|E].
+  - assert (E0:n=(n-n0+n0)) by lia.
+    rewrite E0 in H.
+    epose proof (Steps_split H) as H1.
+    destruct H1 as [st2 [H1a H1b]].
+    exists st2. apply H1a.
+  - specialize (H0 (n0-n)).
+    destruct H0 as [st' H0].
+    exists st'.
+    assert (E1:n0=n0-n+n) by lia.
+    rewrite E1.
+    eapply Steps_trans; eauto 1.
+Qed.
+
+Lemma MoveDist_Steps {tm n st st0 d}:
+  MoveDist tm n st st0 d ->
+  Steps Σ tm n st st0.
+Proof.
+  intros.
+  induction H.
+  1: ctor.
+  ector; eauto 1.
+Qed.
+
+
+Lemma MoveDist_split {tm n1 n2 st st0 d}:
+  MoveDist tm (n1+n2) st st0 d ->
+  exists st1 d1,
+  MoveDist tm n2 st st1 d1 /\
+  MoveDist tm n1 st1 st0 (d-d1).
+Proof.
+gd d. gd st0.
+induction n1; intros.
+- cbn in H.
+  exists st0. exists d.
+  split; auto 1.
+  replace (d-d)%Z with 0%Z by lia.
+  ctor.
+- cbn in H.
+  invst H.
+  specialize (IHn1 _ _ H1).
+  destruct IHn1 as [st1 [d1 [IHn1a IHn1b]]].
+  exists st1. exists d1.
+  split; auto 1.
+  ector; eauto 1.
+  rewrite <-H5. lia.
+Qed.
+
+Lemma MoveDist_minus {tm n1 n2 st st0 st1 d d1}:
+  MoveDist tm (n1+n2) st st0 d ->
+  MoveDist tm n2 st st1 d1 ->
+  MoveDist tm n1 st1 st0 (d-d1).
+Proof.
+  intros.
+  destruct (MoveDist_split H) as [st3 [d3 [H1 H2]]].
+  destruct (MoveDist_unique H1 H0). cg.
+Qed.
+
+Lemma loop1_nonhalt' tm l0 l1 z z0 h0 ls0 ls1 ls2 T d:
+  sidpos_history_WF tm h0 ls0 ->
+  sidpos_history_period h0 ls0 (S (S T)) (S T) ->
+  (l0, z) :: ls1 = skipn (S T) (h0 :: ls0) ->
+  (l1, z0) :: ls2 = skipn (S T) ((l0, z) :: ls1) ->
+  match d with
+  | 0%Z => (z0 =? z)%Z
+  | Z.pos _ => match r l1 with
+               | nil => (z0 <? z)%Z
+               | _ :: _ => false
+               end
+  | Z.neg _ => match l l1 with
+               | nil => (z <? z0)%Z
+               | _ :: _ => false
+               end
+  end = true ->
+  ~ HaltsFromInit Σ Σ0 tm.
+Proof.
+  unfold sidpos_history_WF,sidpos_history_period.
+  intros.
+  assert (A1:(S T)+(S T)<=length ls0). {
+    assert (H0a:S T < S (S T)) by lia.
+    specialize (H0 (S T) H0a). clear H0a.
+    rewrite (nth_error_skipn H1) in H0.
+    rewrite H1 in H2.
+    rewrite skipn_skipn in H2.
+    assert (H4:nth_error (h0 :: ls0) ((S T)+(S T)) <> None) by (epose proof (nth_error_skipn H2); cg).
+    rewrite nth_error_Some in H4. cbn in H4.
+    lia.
+  }
+  assert (A2:(S T)<=length ls0) by lia.
+  eassert (B1:_) by (apply (H (length ls0 - (S T+S T))); lia).
+  eassert (B2:_) by (apply (H (length ls0 - (S T))); lia).
+  replace (length ls0 - (length ls0 - (S T + S T))) with ((S T + S T)) in B1 by lia.
+  replace (length ls0 - (length ls0 - (S T))) with ((S T)) in B2 by lia.
+
+  destruct (nth_error (h0 :: ls0) ((S T + S T))) eqn:E1. 2: contradiction.
+  destruct p as [es1 d1].
+  destruct (nth_error (h0 :: ls0) ((S T))) eqn:E2. 2: contradiction.
+  destruct p as [es2 d2].
+
+  epose proof (MoveDist_Steps B1) as B1'.
+  apply (Steps_NonHalt_trans B1').
+  destruct (ListES_toES es1) as [s1 t1] eqn:Ees1.
+  destruct (ListES_toES es2) as [s2 t2] eqn:Ees2.
+  apply loop1_nonhalt with (n:=S T).
+  1: lia.
+  {
+    clear H3.
+    intros.
+    eassert (D1:_) by (apply (H (length ls0 - (S T+S T)+n0)); lia).
+    eassert (D2:_) by (apply (H (length ls0 - (S T)+n0)); lia).
+
+    replace ((length ls0 - (length ls0 - (S T + S T) + n0))) with (S T + (S T - n0)) in D1 by lia.
+    replace ((length ls0 - (length ls0 - (S T) + n0))) with (S T - n0) in D2 by lia.
+
+    eassert (D3:_) by (apply (H0 ((S T)-n0)); lia).
+    destruct (nth_error (h0 :: ls0) (S T + (S T - n0))). 2: contradiction.
+    destruct (nth_error (h0 :: ls0) ((S T - n0))). 2: contradiction.
+    destruct p as [es3 d3].
+    destruct p0 as [es4 d4].
+    destruct D3 as [D3a D3b].
+
+    replace ((length ls0 - (S T + S T) + n0)) with (n0 + (length ls0 - (S T + S T))) in D1 by lia.
+    epose proof (MoveDist_minus D1 B1) as G1.
+    replace ((length ls0 - (S T) + n0)) with ((S T + n0) + (length ls0 - (S T + S T))) in D2 by lia.
+    epose proof (MoveDist_minus D2 B1) as G2.
+    epose proof (MoveDist_Steps G1) as G1'.
+    epose proof (MoveDist_Steps G2) as G2'.
+    destruct (ListES_toES es3) as [s5 t5] eqn:E3.
+    destruct (ListES_toES es4) as [s6 t6] eqn:E4.
+
+    exists s5. exists t5.
+    exists s6. exists t6.
+    repeat split; auto 1.
+    - destruct es3,es4.
+      cbn in D3a,D3b,E3,E4.
+      invst E3. invst E4.
+      reflexivity.
+    - destruct es3,es4.
+      cbn in D3a,D3b,E3,E4.
+      invst E3. invst E4.
+      reflexivity.
+  }
+  {
+    exists s2. exists t2. exists (d2-d1)%Z.
+    split.
+    1: eapply MoveDist_minus; eauto 1;
+       replace (S T + (length ls0 - (S T + S T))) with (length ls0 - S T) by lia; assumption.
+
+    epose proof (nth_error_skipn H1) as C1.
+    rewrite H1 in H2.
+    rewrite skipn_skipn in H2.
+    epose proof (nth_error_skipn H2) as C2.
+    rewrite E1 in C2.
+    rewrite E2 in C1.
+    invst C1. invst C2. clrs.
+    destruct d.
+    - left. lia.
+    - right. left.
+      destruct l1 as [l' r' m' s'].
+      destruct r' eqn:E3; cbn in H3; cg.
+      split. 1: lia.
+      cbn in Ees1. invst Ees1.
+      unfold half_tape,half_tape_all0,addmul,Dir_to_Z; fext.
+      destruct (1 + 1 * Z.of_nat x)%Z eqn:E3; try lia.
+      destruct (Pos.to_nat p0) eqn:E4; try lia.
+      destruct n; reflexivity.
+    - right. right.
+      destruct l1 as [l' r' m' s'].
+      destruct l' eqn:E3; cbn in H3; cg.
+      split. 1: lia.
+      cbn in Ees1. invst Ees1.
+      unfold half_tape,half_tape_all0,addmul,Dir_to_Z; fext.
+      destruct (-1 + -1 * Z.of_nat x)%Z eqn:E3; try lia.
+      destruct (Pos.to_nat p0) eqn:E4; try lia.
+      destruct n; reflexivity.
+  }
+Qed.
+
+Ltac Σ_eq_dec s1 s2 :=
+  eq_dec Σ_eqb_spec Σ_eqb s1 s2.
+
+Lemma verify_loop1_spec tm h1 h2 ls1 ls2 n d:
+  (exists h0 ls0 n0 n1,
+  sidpos_history_WF tm h0 ls0 /\
+  (h1::ls1) = skipn n0 (h0::ls0) /\
+  (h2::ls2) = skipn (S n1) (h1::ls1) /\
+  sidpos_history_period h0 ls0 n0 (S n1) /\
+  n0+n=(S n1)) ->
+  verify_loop1 h1 h2 ls1 ls2 n d = true ->
+  ~ HaltsFromInit Σ Σ0 tm.
+Proof.
+  gd ls2. gd h2. gd h1. gd n.
+  induction ls1; intros.
+  - cbn in H0.
+    destruct h1,h2.
+    repeat rewrite andb_shortcut_spec in H0.
+    repeat rewrite Bool.andb_true_iff in H0.
+    repeat rewrite orb_shortcut_spec in H0.
+    repeat rewrite Bool.orb_true_iff in H0.
+    destruct H0 as [H0a [H0b [H0c _]]].
+    destruct H as [h0 [ls0 [N [T [Ha [Hb [Hc [Hd He]]]]]]]].
+    destruct n; cg.
+    cbn in Hc. rewrite skipn_nil in Hc. invst Hc.
+  - cbn in H0.
+    destruct h1,h2.
+    repeat rewrite andb_shortcut_spec in H0.
+    repeat rewrite Bool.andb_true_iff in H0.
+    repeat rewrite orb_shortcut_spec in H0.
+    repeat rewrite Bool.orb_true_iff in H0.
+    destruct H0 as [H0a [H0b H0c]].
+
+    destruct H as [h0 [ls0 [N [T [Ha [Hb [Hc [Hd He]]]]]]]].
+    St_eq_dec (s l0) (s l1); cg.
+    Σ_eq_dec (m l0) (m l1); cg.
+    clrs.
+
+    destruct ls2 as [|h2' ls2']; cg.
+    + destruct H0c as [H0c|H0c]; cg.
+      destruct n; cg.
+      epose proof (sidpos_history_period_S Hb Hc Hd H H0).
+      assert (N=S T) by lia; subst.
+      eapply loop1_nonhalt'; eauto 1.
+    + destruct H0c as [H0c|H0c].
+      * destruct n; cg.
+        epose proof (sidpos_history_period_S Hb Hc Hd H H0).
+        assert (N=S T) by lia; subst.
+        eapply loop1_nonhalt'; eauto 1.
+      * destruct n; cbn in H0c.
+        {
+          eapply IHls1; eauto 1.
+          destruct ls0 as [|h0' ls0'].
+          1: destruct N; [lia | cbn in Hb; rewrite skipn_nil in Hb; invst Hb].
+          exists h0'. exists ls0'. exists N. exists T.
+          repeat split; auto 1; try lia.
+          2,3: eapply skipn_S'; eauto 1.
+          1: eapply sidpos_history_WF_cdr,Ha.
+          destruct N as [|N]. 1: lia.
+          epose proof (sidpos_history_period_S' Hd) as Hd'. clear Hd.
+          cbn in Hb.
+          eapply sidpos_history_period_S; eauto 1.
+        }
+        {
+          eapply IHls1; eauto 1.
+          exists h0. exists ls0. exists (S N). exists T.
+          repeat split; auto 1; try lia.
+          1,2: eapply skipn_S; eauto 1.
+          apply (sidpos_history_period_S Hb Hc Hd H H0).
+        }
+Qed.
+
+
+
+Lemma find_loop1_spec tm h0 h1 h2 ls0 ls1 ls2 n:
+  sidpos_history_WF tm h0 ls0 ->
+  h1::ls1 = skipn (S n) (h0::ls0) ->
+  h2::ls2 = skipn (S n) (h1::ls1) ->
+  find_loop1 h0 h1 h2 ls0 ls1 ls2 n = true ->
+  ~ HaltsFromInit Σ Σ0 tm.
+Proof.
+  gd n. gd ls2. gd h2. gd h1.
+  induction ls1.
+  - intros. cbn in H2.
+    cbn in H1. rewrite skipn_nil in H1.
+    invst H1.
+  - intros. cbn in H2.
+    repeat rewrite orb_shortcut_spec in H2.
+    rewrite Bool.orb_true_iff in H2.
+    destruct H2 as [H2|H2].
+    + destruct h0 as [es0 d0].
+      destruct h1 as [es1 d1].
+      destruct h2 as [es2 d2].
+      repeat rewrite andb_shortcut_spec in H2.
+      repeat rewrite Bool.andb_true_iff in H2.
+      destruct H2 as [H2a [H2b [H2c [H2d H2e]]]].
+      eapply verify_loop1_spec; eauto 1.
+      eexists. eexists. exists 0. eexists.
+      repeat split; auto 1.
+      unfold sidpos_history_period. intros. lia.
+    + destruct ls2 as [|h3 [|h2' ls2']]; cg.
+      eapply IHls1; eauto 1.
+      * rewrite (skipn_S H0); cg.
+      * cbn in H1.
+        apply (skipn_S (skipn_S H1)).
+Qed.
+
+
+Lemma find_loop1_0_spec tm h0 h1 ls:
+  sidpos_history_WF tm h0 (h1::ls) ->
+  find_loop1_0 h0 h1 ls = true ->
+  ~HaltsFromInit Σ Σ0 tm.
+Proof.
+  intros.
+  unfold find_loop1_0 in H0.
+  destruct ls; cg.
+  eapply find_loop1_spec; eauto 1; reflexivity.
+Qed.
+
+
+
+Fixpoint loop1_decider0(tm:TM Σ)(n:nat)(es:ListES)(d:Z)(ls:list (ListES*Z))(n0:nat)(ns:list nat):HaltDecideResult :=
+match n with
+| O => Result_Unknown
+| S n0 =>
+  match tm es.(s) es.(m) with
+  | None => Result_Halt es.(s) es.(m)
+  | Some tr =>
+    let es' := ListES_step' tr es in
+    let d' := (d+Dir_to_Z tr.(dir _))%Z in
+    let ls' := ((es,d)::ls) in
+    match n0 with
+    | S n0' =>
+      loop1_decider0 tm n0 es' d' ls' n0' ns
+    | O =>
+      if find_loop1_0 (es',d') (es,d) ls then Result_NonHalt else
+      loop1_decider0 tm n0 es' d' ls' (hd O ns) (tl ns)
+    end
+  end
+end.
+
+Lemma loop1_decider0_def(tm:TM Σ)(n:nat)(es:ListES)(d:Z)(ls:list (ListES*Z))(n0:nat)(ns:list nat):
+loop1_decider0 tm n es d ls n0 ns =
+match n with
+| O => Result_Unknown
+| S n0 =>
+  match tm es.(s) es.(m) with
+  | None => Result_Halt es.(s) es.(m)
+  | Some tr =>
+    let es' := ListES_step' tr es in
+    let d' := (d+Dir_to_Z tr.(dir _))%Z in
+    let ls' := ((es,d)::ls) in
+    match n0 with
+    | S n0' =>
+      loop1_decider0 tm n0 es' d' ls' n0' ns
+    | O =>
+      if find_loop1_0 (es',d') (es,d) ls then Result_NonHalt else
+      loop1_decider0 tm n0 es' d' ls' (hd O ns) (tl ns)
+    end
+  end
+end.
+Proof.
+  unfold loop1_decider0.
+  destruct n; cbn; reflexivity.
+Qed.
+
+Lemma sidpos_history_hd {tm es d ls}:
+  sidpos_history_WF tm (es,d) ls ->
+  MoveDist tm (length ls) (InitES Σ Σ0) (ListES_toES es) d.
+Proof.
+  unfold sidpos_history_WF.
+  intros.
+  specialize (H (length ls)).
+  replace (length ls - length ls) with 0 in H by lia.
+  cbn in H.
+  apply H. lia.
+Qed.
+
+Lemma s_def l0 r0 m0 s0:
+  s {| l:=l0; r:=r0; m:=m0; s:=s0 |} = s0.
+Proof.
+  reflexivity.
+Qed.
+
+Lemma m_def l0 r0 m0 s0:
+  m {| l:=l0; r:=r0; m:=m0; s:=s0 |} = m0.
+Proof.
+  reflexivity.
+Qed.
+
+Lemma sidpos_history_WF_S {tm l0 r0 m0 s0 d ls s1 d1 o1}:
+  sidpos_history_WF tm (Build_ListES l0 r0 m0 s0, d) ls ->
+  tm s0 m0 = Some {| nxt := s1; dir := d1; out := o1 |} ->
+  sidpos_history_WF tm (ListES_step' {| nxt := s1; dir := d1; out := o1 |} (Build_ListES l0 r0 m0 s0), (d+(Dir_to_Z d1))%Z) ((Build_ListES l0 r0 m0 s0, d)::ls).
+Proof.
+  intros.
+  epose proof (ListES_step'_spec tm l0 r0 m0 s0) as H1.
+  remember (Build_ListES l0 r0 m0 s0) as es0.
+  rewrite H0 in H1.
+  remember {| nxt := s1; dir := d1; out := o1 |} as tr.
+  unfold sidpos_history_WF.
+  unfold sidpos_history_WF in H.
+  replace (length ((es0, d) :: ls)) with (S (length ls)) by reflexivity.
+  intros.
+  assert (E:n<=length ls \/ n=S (length ls)) by lia.
+  destruct E as [E|E].
+  - replace (S (length ls) - n) with (S (length ls - n)) by lia.
+    cbn.
+    apply H,E.
+  - replace (S (length ls) - n) with (O) by lia.
+    cbn. rewrite E.
+    eassert (H3:_) by (apply (H (length ls)); lia).
+    rewrite Nat.sub_diag in H3. cbn in H3.
+    subst es0.
+    ector; eauto 1.
+    subst tr. cbn. lia.
+Qed.
+
+Lemma ListES_toES_O:
+  (ListES_toES {| l := nil; r := nil; m := Σ0; s := St0 |}) = InitES Σ Σ0.
+Proof.
+  unfold InitES.
+  cbn.
+  f_equal.
+  fext.
+  destruct x.
+  1: reflexivity.
+  - destruct (Pos.to_nat p).
+    1: reflexivity.
+    destruct n; reflexivity.
+  - destruct (Pos.to_nat p).
+    1: reflexivity.
+    destruct n; reflexivity.
+Qed.
+
+Lemma sidpos_history_WF_O tm:
+  sidpos_history_WF tm ({| l := nil; r := nil; m := Σ0; s := St0 |}, 0%Z) nil.
+Proof.
+  unfold sidpos_history_WF.
+  intros.
+  cbn in H.
+  assert (n=0) by lia. subst.
+  replace (length nil - 0) with 0 by reflexivity.
+  unfold nth_error.
+  rewrite ListES_toES_O.
+  ctor.
+Qed.
+
+Lemma loop1_decider0_spec tm n es d ls n0 ns:
+  sidpos_history_WF tm (es,d) ls ->
+  match loop1_decider0 tm n es d ls n0 ns with
+  | Result_Halt s0 i0 =>
+    exists n1 es0,
+    n1<n+(length ls) /\
+    HaltsAt Σ tm n1 (InitES Σ Σ0) /\
+    Steps Σ tm n1 (InitES Σ Σ0) (ListES_toES es0) /\
+    es0.(s)=s0 /\ es0.(m)=i0
+  | Result_NonHalt => ~HaltsFromInit Σ Σ0 tm
+  | Result_Unknown => True
+  end.
+Proof.
+  gd ns. gd n0. gd ls. gd d. gd es.
+  induction n; intros.
+  1: cbn; trivial.
+  destruct es as [l0 r0 m0 s0] eqn:Ees.
+  rewrite loop1_decider0_def.
+  rewrite s_def,m_def.
+  destruct (tm s0 m0) eqn:E.
+  - rewrite <-Ees.
+    destruct t as [s1 d1 o1].
+    epose proof (sidpos_history_WF_S H E) as H0.
+    rewrite <-Ees in H0.
+    remember {| nxt := s1; dir := d1; out := o1 |} as t.
+    remember (ListES_step' t es) as es'.
+    remember (d + Dir_to_Z (dir Σ t))%Z as d'.
+    remember ((es, d) :: ls) as ls'.
+    destruct n.
+    + cbn.
+      destruct (find_loop1_0 (es', d') (es, d) ls) eqn:E1.
+      2: trivial.
+      eapply find_loop1_0_spec; eauto 1.
+      rewrite Heqt in Heqd'. cbn in Heqd'. subst d'. subst ls'. apply H0.
+    + replace (let es'0 := es' in
+      let d'0 := d' in let ls'0 := ls' in loop1_decider0 tm (S n) es'0 d'0 ls'0 n ns) with
+      (loop1_decider0 tm (S n) es' d' ls' n ns) by reflexivity.
+      specialize (IHn _ _ _ n ns H0).
+      rewrite Heqt in Heqd'. cbn in Heqd'. subst d'. subst ls'.
+      replace (S n + length ((es, d) :: ls)) with (S (S n) + length ls) in IHn by (cbn; lia).
+      apply IHn.
+  - exists (length ls). exists es.
+    repeat split.
+    + lia.
+    + eexists.
+      split.
+      1: apply (MoveDist_Steps (sidpos_history_hd H)).
+      unfold step,ListES_toES. rewrite E. reflexivity.
+    + subst es. apply (MoveDist_Steps (sidpos_history_hd H)).
+    + subst es.  reflexivity.
+    + subst es.  reflexivity.
+Qed.
+
+Fixpoint halt_decider0(tm:TM Σ)(n:nat)(es:ListES):HaltDecideResult :=
+match n with
+| O => Result_Unknown
+| S n0 =>
+  match tm es.(s) es.(m) with
+  | None => Result_Halt es.(s) es.(m)
+  | Some tr => 
+    halt_decider0 tm n0 (ListES_step' tr es)
+  end
+end.
+
+Lemma halt_decider0_spec tm n es n2:
+  Steps Σ tm n2 (InitES Σ Σ0) (ListES_toES es) ->
+  match halt_decider0 tm n es with
+  | Result_Halt s0 i0 =>
+    exists n1 es0,
+    n1<n+n2 /\
+    HaltsAt Σ tm n1 (InitES Σ Σ0) /\
+    Steps Σ tm n1 (InitES Σ Σ0) (ListES_toES es0) /\
+    es0.(s)=s0 /\ es0.(m)=i0
+  | Result_NonHalt => False
+  | Result_Unknown => True
+  end.
+Proof.
+  gd n2. gd es.
+  induction n.
+  - intros.
+    cbn. trivial.
+  - intros.
+    unfold halt_decider0.
+    fold halt_decider0.
+    destruct es as [l0 r0 m0 s0].
+    unfold l,r,m,s.
+    pose proof (ListES_step'_spec tm l0 r0 m0 s0).
+    destruct (tm s0 m0) as [tr|] eqn:E.
+    + assert (Steps Σ tm (S n2) (InitES Σ Σ0) (ListES_toES (ListES_step' tr {| l := l0; r := r0; m := m0; s := s0 |}))) by (ector; eauto 1).
+      specialize (IHn _ _ H1).
+      destruct (halt_decider0 tm n (ListES_step' tr {| l := l0; r := r0; m := m0; s := s0 |})).
+      * destruct IHn as [n1 [es0 IHn]].
+        exists n1. exists es0. destruct es0 as [l2 r2 m2 s2].
+        unfold s,m in IHn.
+        replace (S n + n2) with (n + S n2) by lia.
+        apply IHn.
+      * destruct IHn.
+      * trivial.
+    + exists n2. exists ({| l := l0; r := r0; m := m0; s := s0 |}).
+      repeat split.
+      * lia.
+      * unfold HaltsAt.
+        exists (ListES_toES {| l := l0; r := r0; m := m0; s := s0 |}).
+        split; auto 1.
+      * apply H.
+Qed.
+
+
+
+Definition halt_decider(n:nat)(tm:TM Σ):HaltDecideResult :=
+  halt_decider0 tm n {| l:=nil; r:=nil; m:=Σ0; s:=St0 |}.
+
+Definition loop1_decider(n:nat)(ns:list nat)(tm:TM Σ):HaltDecideResult :=
+  loop1_decider0 tm n {| l:=nil; r:=nil; m:=Σ0; s:=St0 |} Z0 nil (hd O ns) (tl ns).
+
+
+Lemma halt_decider_WF BB n:
+  n<=S BB ->
+  HaltDecider_WF BB (halt_decider n).
+Proof.
+  intros.
+  unfold HaltDecider_WF,halt_decider.
+  intro tm.
+  eassert (H0:_). {
+    apply (halt_decider0_spec tm n {| l := nil; r := nil; m := Σ0; s := St0 |}).
+    rewrite ListES_toES_O.
+    ctor.
+  }
+  destruct (halt_decider0 tm n {| l := nil; r := nil; m := Σ0; s := St0 |}).
+  - destruct H0 as [n0 [es0 [H0 [H1 [H2 [H3 H4]]]]]].
+    destruct es0 as [l0 r0 m0 s1].
+    unfold s,m in H3,H4. subst.
+    exists n0. eexists.
+    repeat split; eauto 1.
+    lia.
+  - contradiction.
+  - trivial.
+Qed.
+
+
+Lemma loop1_decider_WF BB n ns:
+  n<=S BB ->
+  HaltDecider_WF BB (loop1_decider n ns).
+Proof.
+  intros.
+  unfold HaltDecider_WF,loop1_decider.
+  intro tm.
+  eassert (H0:_). {
+    apply (loop1_decider0_spec tm n {| l := nil; r := nil; m := Σ0; s := St0 |} 0 nil (hd 0 ns) (tl ns)).
+    apply sidpos_history_WF_O.
+  }
+  destruct (loop1_decider0 tm n {| l := nil; r := nil; m := Σ0; s := St0 |} 0 nil (hd 0 ns) (tl ns)); auto 1.
+  cbn in H0.
+  destruct H0 as [n1 [es0 [H0 [H1 [H2 [H3 H4]]]]]].
+  destruct (ListES_toES es0) as [s1 t0] eqn:E0.
+  exists n1. exists t0.
+  destruct es0 eqn:E.
+  cbn in E0.
+  inversion E0. subst s2.
+  repeat split; auto 1.
+  2: lia. rewrite <-E0 in H2.
+  cbn in H3,H4. subst.
+  apply H2.
+Qed.
+
+
+Fixpoint ListES_Steps(tm:TM Σ)(n:nat)(es:ListES):option ListES:=
+match n with
+| O => Some es
+| S n0 =>
+  match tm es.(s) es.(m) with
+  | None => None
+  | Some tr =>
+    ListES_Steps tm n0 (ListES_step' tr es)
+  end
+end.
+
+Lemma ListES_Steps_spec tm n es:
+  match ListES_Steps tm n es with
+  | Some es0 => Steps _ tm n (ListES_toES es) (ListES_toES es0)
+  | None => True
+  end.
+Proof.
+  gd es.
+  induction n.
+  1: intro; cbn; ctor.
+  intro.
+  cbn.
+  destruct (tm (s es) (m es)) as [tr|] eqn:E.
+  2: trivial.
+  destruct es as [l0 r0 m0 s0].
+  cbn in E.
+  epose proof (ListES_step'_spec tm l0 r0 m0 s0) as H.
+  rewrite E in H.
+  specialize (IHn (ListES_step' tr {| l := l0; r := r0; m := m0; s := s0 |})).
+  destruct (ListES_Steps tm n (ListES_step' tr {| l := l0; r := r0; m := m0; s := s0 |})).
+  2: trivial.
+  replace (S n) with (n+1) by lia.
+  eapply Steps_trans.
+  2: apply IHn.
+  ector; eauto 1.
+  ctor.
+Qed.
+
+Definition halt_time_verifier(tm:TM Σ)(n:nat):bool :=
+  match ListES_Steps tm n {| l := nil; r := nil; m := Σ0; s := St0 |} with
+  | Some {| l:=_; r:=_; m:=m0; s:=s0 |} =>
+    match tm s0 m0 with
+    | None => true
+    | _ => false
+    end
+  | None => false
+  end.
+
+Lemma halt_time_verifier_spec tm n:
+  halt_time_verifier tm n = true ->
+  HaltsAt _ tm n (InitES Σ Σ0).
+Proof.
+  unfold halt_time_verifier,HaltsAt.
+  intro H.
+  pose proof (ListES_Steps_spec tm n {| l := nil; r := nil; m := Σ0; s := St0 |}).
+  destruct (ListES_Steps tm n {| l := nil; r := nil; m := Σ0; s := St0 |}).
+  2: cg.
+  rewrite ListES_toES_O in H0.
+  eexists.
+  split.
+  - apply H0.
+  - destruct l0 as [l0 r0 m0 s0].
+    cbn.
+    destruct (tm s0 m0); cg.
+Qed.
+
+Definition BB:N := 47176869.
+
+Fixpoint nat_eqb_N(n:nat)(m:N) :=
+match n,m with
+| O,N0 => true
+| S n0,Npos _ => nat_eqb_N n0 (N.pred m)
+| _,_ => false
+end.
+
+Lemma nat_eqb_N_spec n m :
+  nat_eqb_N n m = true -> n = N.to_nat m.
+Proof.
+  gd m.
+  induction n; intros.
+  - cbn in H.
+    destruct m0; cbn; cg.
+  - destruct m0.
+    + cbn in H. cg.
+    + cbn in H.
+      specialize (IHn (Pos.pred_N p) H). lia.
+Qed.
+
+
+Definition halt_decider_max := halt_decider 47176870.
+Lemma halt_decider_max_spec: HaltDecider_WF (N.to_nat BB) halt_decider_max.
+Proof.
+  eapply halt_decider_WF.
+  unfold BB.
+  replace (S (N.to_nat 47176869)) with (N.to_nat 47176870) by lia.
+  replace (Init.Nat.of_num_uint
+    (Number.UIntDecimal
+       (Decimal.D4
+          (Decimal.D7
+             (Decimal.D1
+                (Decimal.D7 (Decimal.D6 (Decimal.D8 (Decimal.D7 (Decimal.D0 Decimal.Nil))))))))))
+  with (N.to_nat 47176870).
+  1: apply Nat.le_refl.
+  symmetry.
+  apply nat_eqb_N_spec.
+  vm_compute.
+  reflexivity.
+Time Qed.
+
+Definition BB5_champion := (makeTM BR1 CL1 CR1 BR1 DR1 EL0 AL1 DL1 HR1 AL0).
+
+Lemma BB5_lower_bound:
+  exists tm,
+  HaltsAt _ tm (N.to_nat BB) (InitES Σ Σ0).
+Proof.
+  exists BB5_champion.
+  apply halt_time_verifier_spec.
+  vm_compute.
+  reflexivity.
+Time Qed.
+
+
+Definition decider0 := HaltDecider_nil.
+Definition decider1 := halt_decider 130.
+Definition decider2 := (loop1_decider 130 (1::2::4::8::16::32::64::128::256::512::nil)).
+
+Definition decider3 := (NGramCPS_decider_impl2 1 1 100).
+Definition decider4 := (NGramCPS_decider_impl2 2 2 200).
+Definition decider5 := (NGramCPS_decider_impl2 3 3 400).
+Definition decider6 := (NGramCPS_decider_impl1 2 2 2 1600).
+Definition decider7 := (NGramCPS_decider_impl1 2 3 3 1600).
+
+Definition decider8 := (loop1_decider 4100 (1::2::4::8::16::32::64::128::256::512::1024::2048::4096::nil)).
+
+Definition decider9 := (NGramCPS_decider_impl1 4 2 2 600).
+Definition decider10 := (NGramCPS_decider_impl1 4 3 3 1600).
+Definition decider11 := (NGramCPS_decider_impl1 6 2 2 3200).
+Definition decider12 := (NGramCPS_decider_impl1 6 3 3 3200).
+Definition decider13 := (NGramCPS_decider_impl1 8 2 2 1600).
+Definition decider14 := (NGramCPS_decider_impl1 8 3 3 1600).
+
+Lemma decider2_WF: HaltDecider_WF (N.to_nat BB) decider2.
+Proof.
+  apply loop1_decider_WF.
+  unfold BB.
+  lia.
+Qed.
+
+Lemma root_q_WF:
+  SearchQueue_WF (N.to_nat BB) root_q root.
+Proof.
+  apply SearchQueue_init_spec,root_WF.
+Qed.
+
+Definition root_q_upd1:=
+  (SearchQueue_upd root_q decider2).
+
+Lemma root_q_upd1_WF:
+  SearchQueue_WF (N.to_nat BB) root_q_upd1 root.
+Proof.
+  apply SearchQueue_upd_spec.
+  - apply root_q_WF.
+  - apply decider2_WF.
+Qed.
+
+Definition first_trans_is_R(x:TNF_Node):bool :=
+  match x.(TNF_tm) St0 Σ0 with
+  | Some {| nxt:=_; dir:=Dpos; out:=_ |} => true
+  | _ => false
+  end.
+
+Definition root_q_upd1_simplified:SearchQueue:=
+  (filter first_trans_is_R (fst root_q_upd1), nil).
+
+Lemma TM_rev_upd'_TM0 s0 o0:
+  (TM_upd' (TM0) St0 Σ0 (Some {| nxt := s0; dir := Dneg; out := o0 |})) =
+  (TM_rev Σ (TM_upd' (TM0) St0 Σ0 (Some {| nxt := s0; dir := Dpos; out := o0 |}))).
+Proof.
+  repeat rewrite TM_upd'_spec.
+  fext. fext.
+  unfold TM_upd,TM_rev,TM0.
+  St_eq_dec x St0.
+  - Σ_eq_dec x0 Σ0; cbn; reflexivity.
+  - cbn; reflexivity.
+Qed.
+
+Lemma root_q_upd1_simplified_WF:
+  SearchQueue_WF (N.to_nat BB) root_q_upd1_simplified root.
+Proof.
+  pose proof (root_q_upd1_WF).
+  cbn in H.
+  destruct H as [Ha Hb].
+  cbn.
+  split.
+  - intros x H0.
+    pose proof (Ha x). tauto.
+  - intro H0. apply Hb.
+    intros x H1.
+    destruct H1 as [H1|[H1|[H1|[H1|[H1|[H1|[H1|[H1|H1]]]]]]]]; try (specialize (H0 x); tauto).
+    1,2,3,4:
+      clear Ha; clear Hb;
+      destruct x as [tm cnt ptr];
+      cbn; invst H1;
+      rewrite TM_rev_upd'_TM0;
+      eapply HaltTimeUpperBound_LE_rev_InitES.
+    1: eassert (H2:_) by (apply (H0 {|
+             TNF_tm := TM_upd' (TM0) St0 Σ0 (Some {| nxt := St0; dir := Dpos; out := Σ0 |});
+             TNF_cnt := 9;
+             TNF_ptr := St1
+           |}); tauto); apply H2.
+    1: eassert (H2:_) by (apply (H0 {|
+             TNF_tm := TM_upd' (TM0) St0 Σ0 (Some {| nxt := St0; dir := Dpos; out := Σ1 |});
+             TNF_cnt := 9;
+             TNF_ptr := St1
+           |}); tauto); apply H2.
+    1: eassert (H2:_) by (apply (H0 {|
+             TNF_tm := TM_upd' (TM0) St0 Σ0 (Some {| nxt := St1; dir := Dpos; out := Σ0 |});
+             TNF_cnt := 9;
+             TNF_ptr := St2
+           |}); tauto); apply H2.
+    1: eassert (H2:_) by (apply (H0 {|
+             TNF_tm := TM_upd' (TM0) St0 Σ0 (Some {| nxt := St1; dir := Dpos; out := Σ1 |});
+             TNF_cnt := 9;
+             TNF_ptr := St2
+           |}); tauto); apply H2.
+Qed.
+
+Fixpoint length_tailrec0{T}(ls:list T)(n:N):N :=
+match ls with
+| nil => n
+| h::t => length_tailrec0 t (N.succ n)
+end.
+Definition length_tailrec{T}(ls:list T):N := length_tailrec0 ls 0.
+
+
+Definition St_to_N(s1:St):N :=
+match s1 with
+| St0 => 1
+| St1 => 2
+| St2 => 3
+| St3 => 4
+| St4 => 5
+end.
+
+Definition Dir_to_N(d1:Dir):N :=
+match d1 with
+| Dpos => 1
+| Dneg => 0
+end.
+
+Definition Σ_to_N(o1:Σ):N :=
+match o1 with
+| Σ0 => 0
+| Σ1 => 1
+end.
+
+Definition Trans_to_N(tr:Trans Σ):list (N*N) :=
+let (s1,d1,o1):=tr in
+((St_to_N s1,6)::(Σ_to_N o1,2)::(Dir_to_N d1,2)::nil)%N.
+
+Definition option_Trans_to_N(tr:option (Trans Σ)):list (N*N) :=
+match tr with
+| None =>
+  ((0,6)::(Σ_to_N Σ1,2)::(Dir_to_N Dpos,2)::nil)%N
+| Some tr => Trans_to_N tr
+end.
+
+Fixpoint TM_to_N_0(ls:list (N*N))(v:N):N :=
+match ls with
+| nil => v
+| (a,b)::t => TM_to_N_0 t (v*b+a)
+end.
+
+Definition TM_to_N(tm:TM Σ):N :=
+  TM_to_N_0 (
+  (option_Trans_to_N (tm St0 Σ0))++
+  (option_Trans_to_N (tm St0 Σ1))++
+  (option_Trans_to_N (tm St1 Σ0))++
+  (option_Trans_to_N (tm St1 Σ1))++
+  (option_Trans_to_N (tm St2 Σ0))++
+  (option_Trans_to_N (tm St2 Σ1))++
+  (option_Trans_to_N (tm St3 Σ0))++
+  (option_Trans_to_N (tm St3 Σ1))++
+  (option_Trans_to_N (tm St4 Σ0))++
+  (option_Trans_to_N (tm St4 Σ1))++nil
+  ) 0.
+
+Definition TNF_Node_list_to_N_list := map (fun (x:TNF_Node) => TM_to_N (TNF_tm x)).
+
+
+Compute (TM_to_N (makeTM BR1 HR1 CL0 ER0 DL0 CL1 AR1 BR0 DR0 DR1)).
+
+End ListTape_assumeSigma.
