Prelims.v
@@ -1,0 +1,75 @@
+Require Import List.
+Require Import ZArith.
+Require Import FSets.FMapPositive.
+
+From BusyCoq Require Import CustomTactics.
+
+Definition is_inj{T1 T2}(f:T1->T2):=
+  forall a b, f a = f b -> a = b.
+
+Lemma fext_inv{A}{B} {f g:A->B}(x:A):
+  f = g ->
+  f x = g x.
+Proof.
+  cg.
+Qed.
+
+Notation "x &&& y" := (if x then y else false) (at level 80, right associativity).
+Notation "x ||| y" := (if x then true else y) (at level 85, right associativity).
+
+Definition set_ins{T}(enc:T->positive)(s:list T * PositiveMap.tree unit)(x:T):(list T * PositiveMap.tree unit)*bool :=
+  let enc := (enc x) in
+  match PositiveMap.find enc (snd s) with
+  | None => ((x::fst s, PositiveMap.add enc tt (snd s)),false)
+  | Some _ => (s,true)
+  end.
+
+Definition set_in{T}(enc:T->positive)(s:list T * PositiveMap.tree unit)(x:T):Prop :=
+  PositiveMap.find (enc x) (snd s) = Some tt.
+
+Definition set_WF{T}(enc:T->positive)(s:list T * PositiveMap.tree unit):Prop :=
+  forall (x:T),
+    set_in enc s x <->
+    In x (fst s).
+
+Lemma set_ins_spec{T} enc (enc_inj: is_inj enc) s (x:T) s' flag:
+  set_WF enc s ->
+  set_ins enc s x = (s',flag) ->
+  (set_WF enc s' /\
+  (flag=true -> (s'=s /\ set_in enc s x))).
+Proof.
+  unfold set_WF,set_ins,set_in.
+  intros.
+  destruct (PositiveMap.find (enc x) (snd s)) as [v|] eqn:E.
+  - invst H0.
+    split.
+    1: assumption.
+    intros.
+    destruct v.
+    split; cg.
+  - invst H0. clear H0.
+    split; intros. 2: cg.
+    cbn.
+    rewrite (PositiveMapAdditionalFacts.gsspec).
+    destruct (PositiveMap.E.eq_dec (enc x0) (enc x)) as [e|e].
+    + pose proof (enc_inj _ _ e); subst.
+      split; tauto.
+    + assert (x<>x0) by cg.
+      split; intro.
+      * right. rewrite <-H. apply H1.
+      * rewrite <-H in H1.
+        destruct H1 as [H1|H1]; cg.
+Qed.
+
+
+
+Lemma empty_set_WF{T}(enc:T->positive):
+  set_WF enc (nil, PositiveMap.empty unit).
+Proof.
+  unfold set_WF.
+  intros. cbn.
+  split; intro.
+  2: contradiction.
+  unfold set_in in H.
+  rewrite PositiveMap.gempty in H. cg.
+Qed.
