TM_CoqBB5.v
@@ -1,0 +1,719 @@
+Require Import ZArith.
+Require Import Lia.
+
+From BusyCoq Require Import Prelims.
+From BusyCoq Require Import BB52Statement.
+From BusyCoq Require Import CustomTactics.
+
+
+Section TM.
+
+Hypothesis Σ:Set.
+Hypothesis Σ0:Σ.
+
+Definition HaltsAt(tm:TM Σ)(n:nat)(st:ExecState Σ): Prop :=
+  exists st', Steps Σ tm n st st' /\ step Σ tm st' = None.
+
+Definition Halts(tm:TM Σ)(st:ExecState Σ): Prop :=
+  exists n, HaltsAt tm n st.
+
+Definition HaltsFromInit(tm:TM Σ): Prop :=
+  Halts tm (InitES Σ Σ0).
+
+Lemma Steps_trans {tm n m st st0 st1}:
+  Steps Σ tm n st st0 ->
+  Steps Σ tm m st0 st1 ->
+  Steps Σ tm (m+n) st st1.
+Proof.
+  intro H.
+  gd st1.
+  induction m; intros; cbn; invst H0.
+  - assumption.
+  - ector; eauto.
+Qed.
+
+Lemma Steps_unique {tm n st st0 st1}:
+  Steps Σ tm n st st0 ->
+  Steps Σ tm n st st1 ->
+  st0 = st1.
+Proof.
+  gd st1.
+  gd st0.
+  induction n; intros st0 st1 H H0; invst H; invst H0.
+  - reflexivity.
+  - specialize (IHn _ _ H2 H3). subst.
+    cg.
+Qed.
+
+Lemma Steps_NonHalt {tm m n st st0}:
+  m<n ->
+  Steps Σ tm n st st0 ->
+  ~HaltsAt tm m st.
+Proof.
+  intros.
+  gd st0.
+  induction n; intros.
+  - lia.
+  - assert (H1:m<n\/m=n) by lia.
+    destruct H1 as [H1|H1].
+    + invst H0.
+      apply (IHn H1 _ H3).
+    + subst.
+      invst H0.
+      unfold HaltsAt,Halts.
+      intro H1.
+      destruct H1 as [st' [H1a H1b]].
+      rewrite <-(Steps_unique H2 H1a) in H1b.
+      destruct st2. cg.
+Qed.
+
+Lemma HaltsAt_unique {tm n1 n2 st}:
+  HaltsAt tm n1 st ->
+  HaltsAt tm n2 st ->
+  n1=n2.
+Proof.
+  intros.
+  pose proof H as H''.
+  pose proof H0 as H0''.
+  unfold HaltsAt in H,H0.
+  pose proof H as H'.
+  pose proof H0 as H0'.
+  destruct H as [st0 [Ha Hb]].
+  destruct H0 as [st1 [H0a H0b]].
+  assert (n1=n2\/n1<n2\/n2<n1) by lia.
+  destruct H as [H|[H|H]]; cg.
+  - destruct (Steps_NonHalt H H0a H'').
+  - destruct (Steps_NonHalt H Ha H0'').
+Qed.
+
+Definition NonHalt tm st :=
+  forall n, exists st', Steps Σ tm n st st'.
+
+Lemma NonHalt_iff {tm st}:
+  NonHalt tm st <-> ~Halts tm st.
+Proof.
+  split; intro.
+  - intro H0.
+    destruct H0 as [n H0].
+    specialize (H (S n)).
+    destruct H as [st' H].
+    eapply Steps_NonHalt.
+    2,3: eassumption.
+    lia.
+  - intro n.
+    induction n.
+    + eexists. ector.
+    + destruct IHn as [st' IHn].
+      unfold Halts,HaltsAt in H.
+      destruct (step Σ tm st') as [st''|] eqn:E.
+      * exists st''. ector; eassumption.
+      * assert False by (apply H; eexists; eexists; split; eassumption).
+        contradiction.
+Qed.
+
+
+Definition LE(tm tm':TM Σ): Prop :=
+  forall (s:St)(i:Σ),
+  tm s i = tm' s i \/
+  tm s i = None.
+
+Lemma LE_step tm tm' st st0:
+  LE tm tm' ->
+  step Σ tm st = Some st0 ->
+  step Σ tm' st = Some st0.
+Proof.
+  unfold LE,step.
+  destruct st as [s t].
+  intros.
+  specialize (H s (t Z0)).
+  destruct (tm s (t Z0)) as [[s' d o]|]; cg.
+  destruct H; cg.
+  rewrite <-H. cg.
+Qed.
+
+Lemma LE_Steps {tm tm' n st st0}:
+  LE tm tm' ->
+  Steps Σ tm n st st0 ->
+  Steps Σ tm' n st st0.
+Proof.
+  intros.
+  induction H0.
+  - ctor.
+  - ector.
+    1: apply IHSteps,H.
+    eapply LE_step; eassumption.
+Qed.
+
+Lemma LE_NonHalts {tm tm' st}:
+  LE tm tm' ->
+  ~Halts tm st ->
+  ~Halts tm' st.
+Proof.
+  repeat rewrite <-NonHalt_iff.
+  unfold NonHalt.
+  intros.
+  destruct (H0 n) as [st' H1].
+  exists st'.
+  eapply LE_Steps; eassumption.
+Qed.
+
+
+Hypothesis BB:nat.
+Definition HaltTimeUpperBound(st:ExecState Σ)(P:TM Σ->Prop):Prop :=
+  forall (tm:TM Σ)(n0:nat), P tm -> HaltsAt tm n0 st -> n0<=BB.
+
+
+Lemma HaltTimeUpperBound_LE_NonHalt {st tm}:
+  ~Halts tm st ->
+  HaltTimeUpperBound st (LE tm).
+Proof.
+  unfold HaltTimeUpperBound.
+  intros.
+  pose proof (LE_NonHalts H0 H) as H2.
+  assert False by (apply H2; eexists; apply H1).
+  contradiction.
+Qed.
+
+Hypothesis Σ_eqb:Σ->Σ->bool.
+Hypothesis Σ_eqb_spec: forall i1 i2, if Σ_eqb i1 i2 then i1=i2 else i1<>i2.
+
+Definition TM_upd tm s i t: TM Σ :=
+  fun s0 i0 =>
+    if (andb (St_eqb s0 s) (Σ_eqb i0 i)) then t else tm s0 i0.
+
+
+Lemma LE_HaltsAtES_1 {tm tm0 n st s t}:
+  LE tm tm0 ->
+  HaltsAt tm n st ->
+  Steps Σ tm n st (s,t) ->
+  tm0 s (t 0%Z) = None ->
+  HaltsAt tm0 n st.
+Proof.
+  intros.
+  unfold HaltsAt.
+  epose proof (LE_Steps H H1).
+  exists (s,t).
+  split. 1: assumption.
+  cbn. rewrite H2. reflexivity.
+Qed.
+
+
+
+Ltac Σ_eq_dec s1 s2 :=
+  eq_dec Σ_eqb_spec Σ_eqb s1 s2.
+
+
+Lemma LE_HaltsAtES_2 {tm tm0 n st s t tr}:
+  LE tm tm0 ->
+  HaltsAt tm n st ->
+  Steps Σ tm n st (s,t) ->
+  tm0 s (t 0%Z) = Some tr ->
+  LE (TM_upd tm s (t 0%Z) (Some tr)) tm0.
+Proof.
+  unfold LE.
+  intros.
+  unfold TM_upd.
+  St_eq_dec s0 s.
+  - Σ_eq_dec i (t Z0); cbn.
+    + left; cg.
+    + apply H.
+  - apply H.
+Qed.
+
+
+Lemma HaltTimeUpperBound_LE_Halt st tm n s t:
+  HaltsAt tm n st ->
+  Steps Σ tm n st (s,t) ->
+  n<=BB ->
+  (forall tr, HaltTimeUpperBound st (LE (TM_upd tm s (t Z0) (Some tr)))) ->
+  HaltTimeUpperBound st (LE tm).
+Proof.
+  intros.
+  unfold HaltTimeUpperBound.
+  intros.
+  destruct (tm0 s (t Z0)) as [tr|] eqn:E.
+  - specialize (H2 tr).
+    eapply H2.
+    2: apply H4.
+    eapply LE_HaltsAtES_2; eassumption.
+  - pose proof (LE_HaltsAtES_1 H3 H H0 E).
+    rewrite (HaltsAt_unique H4 H5).
+    assumption.
+Qed.
+
+
+
+Section swap.
+
+Hypothesis s1 s2:St.
+Hypothesis Hneq12: s1<>s2.
+Hypothesis Hneq01: s1 <> St0.
+Hypothesis Hneq02: s2 <> St0.
+
+Definition St_swap s :=
+  if St_eqb s1 s then s2 else
+  if St_eqb s2 s then s1 else s.
+
+Definition Trans_swap(tr:Trans Σ) :=
+  let (s',d,o):=tr in
+  {| nxt:=St_swap s'; dir:=d; out:=o |}.
+
+Definition option_Trans_swap(x:option (Trans Σ)) :=
+  match x with
+  | Some x0 => Some (Trans_swap x0)
+  | None => None
+  end.
+
+Definition TM_swap(tm:TM Σ) := 
+  fun s i => option_Trans_swap (tm (St_swap s) i).
+
+Definition ExecState_swap(st:ExecState Σ) :=
+  let (s,t):=st in
+  (St_swap s,t).
+
+Lemma St_swap_swap:
+  forall s,
+    St_swap (St_swap s) = s.
+Proof.
+  intros.
+  unfold St_swap.
+  St_eq_dec s1 s;St_eq_dec s2 s;St_eq_dec s1 s2; auto; try cg.
+  - St_eq_dec s2 s2; cg.
+  - St_eq_dec s1 s1; cg.
+  - St_eq_dec s1 s; try cg.
+    St_eq_dec s2 s; try cg.
+Qed.
+
+Lemma Trans_swap_swap:
+  forall t,
+    Trans_swap (Trans_swap t) = t.
+Proof.
+  intros.
+  destruct t.
+  unfold Trans_swap.
+  f_equal.
+  apply St_swap_swap.
+Qed.
+
+Lemma option_Trans_swap_swap:
+  forall s,
+    option_Trans_swap (option_Trans_swap s) = s.
+Proof.
+  intros.
+  destruct s; auto 1.
+  unfold option_Trans_swap. f_equal.
+  apply Trans_swap_swap.
+Qed.
+
+Lemma TM_swap_swap:
+  forall tm,
+    TM_swap (TM_swap tm) = tm.
+Proof.
+  intros.
+  unfold TM_swap.
+  fext. fext.
+  rewrite option_Trans_swap_swap,St_swap_swap.
+  reflexivity.
+Qed.
+
+Lemma ExecState_swap_swap:
+  forall st,
+    ExecState_swap (ExecState_swap st) = st.
+Proof.
+  intros.
+  destruct st as [s t].
+  unfold ExecState_swap.
+  f_equal.
+  apply St_swap_swap.
+Qed.
+
+
+
+
+Lemma step_swap {tm st st0}:
+  step Σ (TM_swap tm) st = Some st0 <->
+  step Σ tm (ExecState_swap st) = Some (ExecState_swap st0).
+Proof.
+  destruct st,st0. cbn.
+  unfold TM_swap.
+  destruct (tm (St_swap s) (σ 0%Z)) eqn:E; cbn.
+  2: split; intro; cg.
+  destruct t. cbn.
+  split; intro; f_equal.
+  - invst H.
+    f_equal.
+    rewrite St_swap_swap; reflexivity.
+  - invst H.
+    f_equal.
+    apply St_swap_swap.
+Qed.
+
+Lemma step_halt_swap tm st:
+  step Σ (TM_swap tm) st = None <->
+  step Σ tm (ExecState_swap st) = None.
+Proof.
+  destruct st. cbn.
+  unfold TM_swap.
+  destruct (tm (St_swap s) (σ 0%Z)) eqn:E; cbn.
+  2: split; intro; cg.
+  destruct t. cbn.
+  split; intro; cg.
+Qed.
+
+
+Lemma Steps_swap tm n st st0:
+  Steps Σ (TM_swap tm) n st st0 <->
+  Steps Σ tm n (ExecState_swap st) (ExecState_swap st0).
+Proof.
+gd st0.
+induction n; intros.
+- split; intros; invst H.
+  + ctor.
+  + ff_inj ExecState_swap_swap H1.
+    ctor.
+- split; intros.
+  + invst H.
+    rewrite IHn in H1.
+    ector; eauto.
+    apply step_swap,H3.
+  + invst H.
+    pose proof (IHn (ExecState_swap st2)) as IHn'.
+    rewrite ExecState_swap_swap in IHn'.
+    rewrite <-IHn' in H1.
+    ector; eauto.
+    apply step_swap.
+    rewrite ExecState_swap_swap.
+    apply H3.
+Qed.
+
+
+Lemma LE_swap_0 tm tm':
+  LE tm tm' -> LE (TM_swap tm) (TM_swap tm').
+Proof.
+  unfold LE.
+  intros.
+  unfold TM_swap.
+  specialize (H (St_swap s) i).
+  destruct H as [H|H]; rewrite H; tauto.
+Qed.
+
+Lemma LE_swap tm tm':
+  LE tm tm' <-> LE (TM_swap tm) (TM_swap tm').
+Proof.
+  split.
+  - apply LE_swap_0.
+  - pose proof (LE_swap_0 (TM_swap tm) (TM_swap tm')) as H.
+    repeat rewrite TM_swap_swap in H.
+    apply H.
+Qed.
+
+Lemma InitES_swap:
+  ExecState_swap (InitES Σ Σ0) = InitES Σ Σ0.
+Proof.
+  unfold InitES. cbn.
+  f_equal.
+  unfold St_swap.
+  St_eq_dec s1 St0; try cg.
+  St_eq_dec s2 St0; try cg.
+Qed.
+
+Lemma HaltsAt_swap_0 tm n st:
+  HaltsAt tm n st ->
+  HaltsAt (TM_swap tm) n (ExecState_swap st).
+Proof.
+  unfold HaltsAt.
+  intros.
+  destruct H as [st' [H H0]].
+  eexists.
+  split.
+  - rewrite Steps_swap.
+    rewrite <-ExecState_swap_swap in H.
+    rewrite ExecState_swap_swap.
+    apply H.
+  - rewrite step_halt_swap,ExecState_swap_swap.
+    apply H0.
+Qed.
+
+Lemma HaltsAt_swap tm n st:
+  HaltsAt tm n st <->
+  HaltsAt (TM_swap tm) n (ExecState_swap st).
+Proof.
+  split.
+  - apply HaltsAt_swap_0.
+  - pose proof (HaltsAt_swap_0 (TM_swap tm) n (ExecState_swap st)) as H.
+    rewrite TM_swap_swap,ExecState_swap_swap in H.
+    apply H.
+Qed.
+
+Lemma HaltTimeUpperBound_LE_swap tm st:
+  HaltTimeUpperBound st (LE tm) -> HaltTimeUpperBound (ExecState_swap st) (LE (TM_swap tm)).
+Proof.
+  unfold HaltTimeUpperBound.
+  intros.
+  rewrite LE_swap,TM_swap_swap in H0.
+  eapply H.
+  1: apply H0.
+  rewrite <-ExecState_swap_swap.
+  rewrite <-HaltsAt_swap.
+  apply H1.
+Qed.
+
+Lemma HaltTimeUpperBound_LE_swap_InitES tm:
+  HaltTimeUpperBound (InitES Σ Σ0) (LE tm) -> HaltTimeUpperBound (InitES Σ Σ0) (LE (TM_swap tm)).
+Proof.
+  intro.
+  rewrite <-InitES_swap.
+  apply HaltTimeUpperBound_LE_swap,H.
+Qed.
+
+End swap.
+
+
+
+Section rev.
+Definition Trans_rev(tr:Trans Σ) :=
+  let (s',d,o):=tr in
+  {| nxt:=s'; dir:=Dir_rev d; out:=o |}.
+
+Definition option_Trans_rev(o:option (Trans Σ)) :=
+  match o with
+  | None => None
+  | Some tr => Some (Trans_rev tr)
+  end.
+
+Definition TM_rev(tm:TM Σ) := 
+  fun s i => option_Trans_rev (tm s i).
+
+Definition Tape_rev(t:Z->Σ) :=
+  fun x:Z => t (-x)%Z.
+
+Definition ExecState_rev(st:ExecState Σ) :=
+  let (s,t):=st in
+  (s,Tape_rev t).
+
+
+Lemma Trans_rev_rev:
+  forall t,
+    Trans_rev (Trans_rev t) = t.
+Proof.
+  intros.
+  destruct t.
+  unfold Trans_rev.
+  f_equal.
+  destruct dir; auto.
+Qed.
+
+Lemma option_Trans_rev_rev:
+  forall t,
+    option_Trans_rev (option_Trans_rev t) = t.
+Proof.
+  intros.
+  destruct t.
+  2: reflexivity.
+  cbn.
+  f_equal.
+  apply Trans_rev_rev.
+Qed.
+
+Lemma TM_rev_rev:
+  forall tm,
+    TM_rev (TM_rev tm) = tm.
+Proof.
+  intros.
+  unfold TM_rev.
+  fext. fext.
+  apply option_Trans_rev_rev.
+Qed.
+
+Lemma Tape_rev_rev:
+  forall t,
+    Tape_rev (Tape_rev t) = t.
+Proof.
+  intros.
+  unfold Tape_rev.
+  fext. f_equal.
+  lia.
+Qed.
+
+Lemma ExecState_rev_rev:
+  forall st,
+    ExecState_rev (ExecState_rev st) = st.
+Proof.
+  intros.
+  destruct st as [s t].
+  cbn.
+  f_equal.
+  apply Tape_rev_rev.
+Qed.
+
+
+
+Lemma step_rev tm st st0:
+  step Σ (TM_rev tm) st = Some st0 <->
+  step Σ tm (ExecState_rev st) = Some (ExecState_rev st0).
+Proof.
+  destruct st,st0. cbn.
+  unfold Tape_rev. cbn.
+  unfold TM_rev.
+  destruct (tm s (σ 0%Z)) as [[s' d o]|] eqn:E; cbn.
+  2: split; intro; cg.
+  split; intro.
+  - invst H.
+    f_equal; f_equal.
+    unfold mov. fext.
+    unfold upd.
+    destruct d; cbn.
+    + assert (x=1\/x<>1)%Z by lia;
+      destruct H0;
+      destruct ((x + -1 =? 0)%Z) eqn:E0; 
+      destruct ((-x + 1 =? 0)%Z) eqn:E1; try lia; cg.
+      f_equal; lia.
+    + assert (x=-1\/x<>-1)%Z by lia;
+      destruct H0;
+      destruct ((x + 1 =? 0)%Z) eqn:E0; 
+      destruct ((-x + -1 =? 0)%Z) eqn:E1; try lia; cg.
+      f_equal; lia.
+  - invst H.
+    f_equal; f_equal.
+    unfold mov.
+    unfold mov in H2.
+    fext.
+    pose proof (fext_inv (-x)%Z H2) as H3.
+    cbn in H3.
+    assert ((- - x)%Z = x) by lia.
+    rewrite H0 in H3.
+    rewrite <-H3.
+    destruct d; cbn.
+    + unfold upd.
+      assert (H1:(x=-1\/x<>-1)%Z) by lia.
+      destruct H1;
+      destruct ((x + 1 =? 0)%Z) eqn:E0;
+      destruct ((-x + -1 =? 0)%Z) eqn:E1; try lia; cg.
+      f_equal; lia.
+    + unfold upd.
+      assert (H4:(x=1\/x<>1)%Z) by lia;
+      destruct H4;
+      destruct ((x + -1 =? 0)%Z) eqn:E0; 
+      destruct ((-x + 1 =? 0)%Z) eqn:E1; try lia; cg.
+      f_equal; lia.
+Qed.
+
+
+Lemma step_halt_rev tm st:
+  step Σ (TM_rev tm) st = None <->
+  step Σ tm (ExecState_rev st) = None.
+Proof.
+  destruct st.
+  cbn.
+  unfold Tape_rev.
+  cbn.
+  unfold TM_rev.
+  destruct (tm s (σ 0%Z)) eqn:E; cbn.
+  2: tauto.
+  destruct t; cbn.
+  split; intro; cg.
+Qed.
+
+Lemma Steps_rev tm n st st0:
+  Steps Σ (TM_rev tm) n st st0 <->
+  Steps Σ tm n (ExecState_rev st) (ExecState_rev st0).
+Proof.
+gd st0.
+induction n; intros.
+- split; intros; invst H.
+  + ctor.
+  + ff_inj ExecState_rev_rev H1.
+    ctor.
+- split; intros.
+  + invst H.
+    rewrite IHn in H1.
+    ector; eauto.
+    apply step_rev,H3.
+  + invst H.
+    pose proof (IHn (ExecState_rev st2)) as IHn'.
+    rewrite ExecState_rev_rev in IHn'.
+    rewrite <-IHn' in H1.
+    ector; eauto.
+    apply step_rev.
+    rewrite ExecState_rev_rev.
+    apply H3.
+Qed.
+
+Lemma LE_rev_0 tm tm':
+  LE tm tm' -> LE (TM_rev tm) (TM_rev tm').
+Proof.
+  unfold LE.
+  intros.
+  unfold TM_rev.
+  pose proof (H s i) as H0.
+  destruct H0 as [H0|H0]; rewrite H0; tauto.
+Qed.
+
+Lemma LE_rev tm tm':
+  LE tm tm' <-> LE (TM_rev tm) (TM_rev tm').
+Proof.
+  split.
+  - apply LE_rev_0.
+  - pose proof (LE_rev_0 (TM_rev tm) (TM_rev tm')) as H.
+    repeat rewrite TM_rev_rev in H.
+    apply H.
+Qed.
+
+Lemma InitES_rev:
+  ExecState_rev (InitES Σ Σ0) = InitES Σ Σ0.
+Proof.
+  reflexivity.
+Qed.
+
+Lemma HaltsAt_rev_0 tm n st:
+  HaltsAt tm n st ->
+  HaltsAt (TM_rev tm) n (ExecState_rev st).
+Proof.
+  unfold HaltsAt.
+  intros.
+  destruct H as [st' [H H0]].
+  eexists.
+  split.
+  - rewrite Steps_rev.
+    rewrite <-ExecState_rev_rev in H.
+    rewrite ExecState_rev_rev.
+    apply H.
+  - rewrite step_halt_rev,ExecState_rev_rev.
+    apply H0.
+Qed.
+
+Lemma HaltsAt_rev tm n st:
+  HaltsAt tm n st <->
+  HaltsAt (TM_rev tm) n (ExecState_rev st).
+Proof.
+  split.
+  - apply HaltsAt_rev_0.
+  - pose proof (HaltsAt_rev_0 (TM_rev tm) n (ExecState_rev st)) as H.
+    rewrite TM_rev_rev,ExecState_rev_rev in H.
+    apply H.
+Qed.
+
+Lemma HaltTimeUpperBound_LE_rev tm st:
+  HaltTimeUpperBound st (LE tm) -> HaltTimeUpperBound (ExecState_rev st) (LE (TM_rev tm)).
+Proof.
+  unfold HaltTimeUpperBound.
+  intros.
+  rewrite LE_rev,TM_rev_rev in H0.
+  eapply H.
+  1: apply H0.
+  rewrite <-ExecState_rev_rev.
+  rewrite <-HaltsAt_rev.
+  apply H1.
+Qed.
+
+Lemma HaltTimeUpperBound_LE_rev_InitES tm:
+  HaltTimeUpperBound (InitES Σ Σ0) (LE tm) -> HaltTimeUpperBound (InitES Σ Σ0) (LE (TM_rev tm)).
+Proof.
+  intro.
+  rewrite <-InitES_rev.
+  apply HaltTimeUpperBound_LE_rev,H.
+Qed.
+
+End rev.
+
+End TM.
